\section{The Einstein-Hilbert Action in the Form Language}

We'll begin with a quick recap of the vielbein/spin connection formalism, for now we'll keep the discussion general in $D$ dimensions, and 
only later on we'll go to the special case of $D=2+1$. The whole point of introducing the Vielbein is switch the degrees of freedom from the 
metric to the inertial frame basis, that is, the vielbein are a collection of $D$ vector fields, such that at each point these collection of 
vectors constitute a basis of the tangent vector space, we'll use the Wald conventions, that is, the ``\textit{true}'' indices which indexes 
which vector field we're talking about $\mu$, and the coordinate basis index $a$,
\begin{align*}
    \textnormal{diag}\mqty(-1& 1&\cdots&1)=\eta_{\mu\nu}&=\vb g\qty(\vb e_\mu,\vb e_\nu)=g_{ab}\dd{x^a}\qty(\vb e_\mu)\otimes\dd{x^b}\qty(\vb e_\nu)\\
    \eta_{\mu\nu}&=g_{ab}\tensor{e}{_\mu^c}\tensor{e}{_\nu^d}\dd{x^a}\qty(\boldsymbol\partial_c)\otimes\dd{x^b}\qty(\boldsymbol\partial_d)\\
    \eta_{\mu\nu}&=g_{ab}\tensor{e}{_\mu^a}\tensor{e}{_\nu^b}
\end{align*}

From the condition that $\vb g$ must be non-degenerate we get that the matrix of components $\tensor{e}{_\mu^a}$ must be invertible, this ensures 
the existence of $\tensor{e}{^\mu_a}$ from which we can construct the dual vector field $\tilde{\vb e}^\mu=\tensor{e}{^\mu_a}\dd{x^a}$ this ensures 
we have a basis of the whole tensor space, so it's possible to decompose any tensor in it,
\begin{align*}
    \eta_{\mu\nu}\tilde{\vb e}^\mu\otimes\tilde{\vb e}^\nu&=\vb g\qty(\vb e_\mu,\vb e_\nu)\tilde{\vb e}^\mu\otimes\tilde{\vb e}^\nu=\vb g
\end{align*}

Only having a metric, or in this case, only having a vielbein, isn't sufficient to construct a theory, we also need a affine connection/covariant 
derivative. A useful way to define it is to define in a vector field basis, as we already have the vielbein as a vector field basis it's more 
convenient to define in respect to it,
\begin{align*}
    \nabla_{\vb X}\qty(\vb e_\nu)&=\tensor{{\boldsymbol\omega(\vb X)}}{^\mu_\nu}\vb e_\mu\\
    \nabla_{\vb X}\qty(\vb e_\nu)&=X^a\tensor{\omega}{_a^\mu_\nu}\vb e_\mu
\end{align*}

Where $\tensor{{\boldsymbol\omega}}{^\mu_\nu}=\tensor{\omega}{_a^\mu_\nu}\dd{x^a}$ is the spin connection, it can be seen as a $\mathfrak{gl}\qty(1,D-1;\mathbb R)$-valued $(0,1)$ tensor, 
or, as we'll adopt here, a $\mathfrak{gl}\qty(1,D-1;\mathbb R)$-valued $1$-form. The ease of working with the vielbein is that the Lorentz index $\mu$ 
does not change upon coordinate/chart/diffeomorphism transformations, and it acts as if it was an internal symmetry, notice that we have a 
redundancy of how to choose the vielbein basis, due to $\tensor{\Lambda}{^\mu_\nu}\vb e_\mu$, $\tensor{\Lambda}{^\mu_\nu}:M\rightarrow\mathbb R$, being an equally good basis,
\begin{align*}
    \vb g\qty(\tensor{\Lambda}{^\alpha_\mu}\vb e_\alpha,\tensor{\Lambda}{^\beta_\nu}\vb e_\beta)&=\tensor{\Lambda}{^\alpha_\mu}\tensor{\Lambda}{^\beta_\nu}\vb g\qty(\vb e_\alpha,\vb e_\beta)\\
    \vb g\qty(\tensor{\Lambda}{^\alpha_\mu}\vb e_\alpha,\tensor{\Lambda}{^\beta_\nu}\vb e_\beta)&=\tensor{\Lambda}{^\alpha_\mu}\tensor{\Lambda}{^\beta_\nu}\eta_{\alpha\beta}\\
    \vb g\qty(\tensor{\Lambda}{^\alpha_\mu}\vb e_\alpha,\tensor{\Lambda}{^\beta_\nu}\vb e_\beta)&=\eta_{\mu\nu}
\end{align*}
as long as $\tensor{\Lambda}{^\alpha_\mu}\tensor{\Lambda}{^\beta_\nu}\eta_{\alpha\beta}=\eta_{\mu\nu}$, that is, as we enlarge the number of components going from the metric to 
the vielbein, we also enlarge the redundancies, now, additionally to Diff$\qty(M)$ we have local $SO\qty(1,D-1)$ transformations as redundancies, this is as 
we was gauging the whole Poincar√© group, with Diff$\qty(M)$ being the gauging of the translations.

\begin{align*}
    \vb g\qty(\vb e_\alpha,\nabla_{\vb X}\qty(\vb e_\nu))&=X^a\tensor{\omega}{_a^\mu_\nu}\vb g\qty(\vb e_\alpha,\vb e_\mu)\\
    \vb g\qty(\vb e_\alpha,\nabla_{\vb X}\qty(\vb e_\nu))+\vb g\qty(\vb e_\nu,\nabla_{\vb X}\qty(\vb e_\alpha))&=X^a\tensor{\omega}{_a^\mu_\nu}\vb g\qty(\vb e_\alpha,\vb e_\mu)+X^a\tensor{\omega}{_a^\mu_\alpha}\vb g\qty(\vb e_\nu,\vb e_\mu)\\
    \vb g\qty(\vb e_\alpha,\nabla_{\vb X}\qty(\vb e_\nu))+\vb g\qty(\nabla_{\vb X}\qty(\vb e_\alpha),\vb e_\nu)&=X^a\tensor{\omega}{_a_\alpha_\nu}+X^a\tensor{\omega}{_a_\nu_\alpha}\\
    \nabla_{\vb X}\qty(\vb g\qty(\vb e_\alpha,\vb e_\nu))-\nabla_{\vb X}\qty(\vb g)\qty(\vb e_\alpha,\vb e_\nu)&=X^a\tensor{\omega}{_a_\alpha_\nu}+X^a\tensor{\omega}{_a_\nu_\alpha}\\
    -\nabla_{\vb X}\qty(\vb g)\qty(\vb e_\alpha,\vb e_\nu)&=X^a\tensor{\omega}{_a_\alpha_\nu}+X^a\tensor{\omega}{_a_\nu_\alpha}\\
    -\tensor{\omega}{_a_\nu_\alpha}&=\tensor{\omega}{_a_\alpha_\nu},\ \ \ \textnormal{Metric compatibility}\numberthis
\end{align*}

Riemann curvature tensor, $\textbf{Riem}\qty(\vb X,\vb Y):\mathfrak X\rightarrow\mathfrak X$:

\begin{align*}
    \textbf{Riem}\qty(\vb X,\vb Y)\vb e_\mu&=\qty(\nabla_{\vb X}\nabla_{\vb Y}-\nabla_{\vb Y}\nabla_{\vb X}-\nabla_{\comm{\vb X}{\vb Y}})\vb e_\mu\\
    \textbf{Riem}\qty(\vb X,\vb Y)\vb e_\mu&=\qty(\nabla_{\vb X}\qty(Y^b\tensor{\omega}{_b^\nu_\mu}\vb e_\nu)-\nabla_{\vb Y}\qty(X^a\tensor{\omega}{_a^\nu_\mu}\vb e_\nu)-\comm{\vb X}{\vb Y}^b\tensor{\omega}{_b^\nu_\mu}\vb e_\nu)\\
    \textbf{Riem}\qty(\vb X,\vb Y)\vb e_\mu&=\qty(\nabla_{\vb X}\qty(Y^b\tensor{\omega}{_b^\nu_\mu}\vb e_\nu)-\nabla_{\vb Y}\qty(X^a\tensor{\omega}{_a^\nu_\mu}\vb e_\nu)-\comm{\vb X}{\vb Y}^b\tensor{\omega}{_b^\nu_\mu}\vb e_\nu)\\
    \textbf{Riem}\qty(\vb X,\vb Y)\vb e_\mu&=\left(Y^b\nabla_{\vb X}\qty(\tensor{\omega}{_b^\nu_\mu}\vb e_\nu)-X^a\nabla_{\vb Y}\qty(\tensor{\omega}{_a^\nu_\mu}\vb e_\nu)\right.\\
    &\quad\quad\quad\left.+\nabla_{\vb X}\qty(Y^b)\tensor{\omega}{_b^\nu_\mu}\vb e_\nu-\nabla_{\vb Y}\qty(X^b)\tensor{\omega}{_b^\nu_\mu}\vb e_\nu-\comm{\vb X}{\vb Y}^b\tensor{\omega}{_b^\nu_\mu}\vb e_\nu\right)\\
    \textbf{Riem}\qty(\vb X,\vb Y)\vb e_\mu&=\left(X^aY^b\nabla_{a}\qty(\tensor{\omega}{_b^\nu_\mu}\vb e_\nu)-X^aY^b\nabla_{b}\qty(\tensor{\omega}{_a^\nu_\mu}\vb e_\nu)\right.\\
    &\quad\quad\quad\left.+\qty(\nabla_{\vb X}\qty(Y^b)-\nabla_{\vb Y}\qty(X^b))\tensor{\omega}{_b^\nu_\mu}\vb e_\nu-\comm{\vb X}{\vb Y}^b\tensor{\omega}{_b^\nu_\mu}\vb e_\nu\right)\\
    \textbf{Riem}\qty(\vb X,\vb Y)\vb e_\mu&=\left(X^aY^b\nabla_{a}\qty(\tensor{\omega}{_b^\nu_\mu})\vb e_\nu+X^aY^b\tensor{\omega}{_b^\nu_\mu}\tensor{\omega}{_a^\alpha_\nu}\vb e_\alpha-X^aY^b\nabla_{b}\qty(\tensor{\omega}{_a^\nu_\mu})\vb e_\nu-X^aY^b\tensor{\omega}{_a^\nu_\mu}\tensor{\omega}{_b^\alpha_\nu}\vb e_\alpha)\right.\\
    &\quad\quad\quad\left.+\qty(X^a\partial_a Y^b+X^a\tensor{\Gamma}{_a^b_c}Y^c-Y^a\partial_aX^b-Y^a\tensor{\Gamma}{_a^b_c}X^c)\tensor{\omega}{_b^\nu_\mu}\vb e_\nu-\qty(X^a\partial_aY^b-Y^a\partial_a X^b)\tensor{\omega}{_b^\nu_\mu}\vb e_\nu\right)\\
    \textbf{Riem}\qty(\vb X,\vb Y)\vb e_\mu&=X^aY^b\left(\nabla_{a}\qty(\tensor{\omega}{_b^\nu_\mu})+\tensor{\omega}{_b^\alpha_\mu}\tensor{\omega}{_a^\nu_\alpha}-\nabla_{b}\qty(\tensor{\omega}{_a^\nu_\mu})-\tensor{\omega}{_a^\alpha_\mu}\tensor{\omega}{_b^\nu_\alpha}+\tensor{\Gamma}{_a^c_b}\tensor{\omega}{_c^\nu_\mu}-\tensor{\Gamma}{_b^c_a}\tensor{\omega}{_c^\nu_\mu}\right)\vb e_\nu\\
    \textbf{Riem}\qty(\vb X,\vb Y)\vb e_\mu&=X^aY^b\left(\partial_{a}\tensor{\omega}{_b^\nu_\mu}-\partial_{b}\tensor{\omega}{_a^\nu_\mu}+\tensor{\omega}{_a^\nu_\alpha}\tensor{\omega}{_b^\alpha_\mu}-\tensor{\omega}{_b^\nu_\alpha}\tensor{\omega}{_a^\alpha_\mu}\right)\vb e_\nu\\
    \textbf{Riem}\qty(\vb X,\vb Y)\vb e_\mu&=X^aY^b\tensor{\left(\dd{\boldsymbol\omega}+\boldsymbol\omega\wedge\boldsymbol\omega\right)}{_a_b^\nu_\mu}\vb e_\nu\\
    \textbf{Riem}\qty(\vb X,\vb Y)\vb e_\mu&=X^aY^b\tensor{R}{_a_b^\nu_\mu}\vb e_\nu\\
    \textbf{Riem}\qty(\vb X,\vb Y)\qty(\tensor{e}{_\mu^e}\boldsymbol\partial_e)&=X^aY^b\tensor{R}{_a_b^\nu_\mu}\tensor{e}{_\nu^c}\boldsymbol\partial_c\\
    \tensor{e}{_\mu^e}\textbf{Riem}\qty(\vb X,\vb Y)\boldsymbol\partial_e&=X^aY^b\tensor{R}{_a_b^\nu_\mu}\tensor{e}{_\nu^c}\boldsymbol\partial_c\\
    \tensor{e}{_\mu^e}X^aY^b\tensor{R}{_a_b^c_e}\boldsymbol\partial_c&=X^aY^b\tensor{R}{_a_b^\nu_\mu}\tensor{e}{_\nu^c}\boldsymbol\partial_c\\
    \tensor{e}{^\mu_d}\tensor{e}{_\mu^e}\tensor{R}{_a_b^c_e}&=\tensor{e}{^\mu_d}\tensor{R}{_a_b^\nu_\mu}\tensor{e}{_\nu^c}\\
    \tensor{R}{_a_b^c_d}&=\tensor{e}{^\mu_d}\tensor{R}{_a_b^\nu_\mu}\tensor{e}{_\nu^c}
\end{align*}

We would like to write the Einstein-Hilbert action as only a function of the Vierbein and the spin connection, for this, let us explicit write the Riemann tensor as a End$\qty(\textnormal TM)$-valued 2-form,

\begin{align*}
    \tensor{{\vb R}}{^\nu_\mu}&=\frac12\tensor{R}{_a_b^\nu_\mu}\dd{x^a}\wedge\dd{x^b}\\
    \tensor{{\vb R}}{^\nu_\mu}&=\frac12\tensor{R}{_a_b^\nu_\mu}\tensor{e}{_\alpha^a}\tensor{e}{^\alpha_c}\tensor{e}{_\beta^b}\tensor{e}{^\beta_d}\dd{x^c}\wedge\dd{x^d}\\
    \tensor{{\vb R}}{^\nu_\mu}&=\frac12\tensor{R}{_a_b^\nu_\mu}\tensor{e}{_\alpha^a}\tensor{e}{_\beta^b}{\tilde{\vb e}^\alpha}\wedge{\tilde{\vb e}^\beta}
\end{align*}

Let us start by writing the volume form in terms of the Vierbein,

\begin{align*}
    \dd[D]{x}\sqrt{\abs{g}}&=\sqrt{\abs{\Det\qty[g_{ab}]}}\dd{x^0}\wedge\cdots\wedge\dd{x^{D-1}}\\
    \dd[D]{x}\sqrt{\abs{g}}&=\sqrt{\abs{\Det\qty[\tensor{e}{^\mu_a}\eta_{\mu\nu}\tensor{e}{^\nu_b}]}}\dd{x^0}\wedge\cdots\wedge\dd{x^{D-1}}\\
    \dd[D]{x}\sqrt{\abs{g}}&=\sqrt{\abs{\Det\qty[\tensor{e}{^\mu_a}]\Det\qty[\eta_{\mu\nu}]\Det\qty[\tensor{e}{^\nu_b}]}}\dd{x^0}\wedge\cdots\wedge\dd{x^{D-1}}\\
    \dd[D]{x}\sqrt{\abs{g}}&=\sqrt{\qty(\Det\qty[\tensor{e}{^\mu_a}])^2}\dd{x^0}\wedge\cdots\wedge\dd{x^{D-1}}\\
    \dd[D]{x}\sqrt{\abs{g}}&=\Det\qty[\tensor{e}{^\mu_a}]\dd{x^0}\wedge\cdots\wedge\dd{x^{D-1}}\\
    \dd[D]{x}\sqrt{\abs{g}}&=\epsilon_{\mu_0\cdots\mu_{D-1}}\tensor{e}{^{\mu_0}_0}\cdots\tensor{e}{^{\mu_{D-1}}_{D-1}}\dd{x^0}\wedge\cdots\wedge\dd{x^{D-1}}\\
    \dd[D]{x}\sqrt{\abs{g}}&=\epsilon_{\mu_0\cdots\mu_{D-1}}\tensor{e}{^{\mu_0}_0}\dd{x^0}\wedge\cdots\wedge\tensor{e}{^{\mu_{D-1}}_{D-1}}\dd{x^{D-1}}\\
    \dd[D]{x}\sqrt{\abs{g}}&=\frac{1}{D!}\epsilon_{\mu_0\cdots\mu_{D-1}}\tensor{e}{^{\mu_0}_{a_0}}\dd{x^{a_0}}\wedge\cdots\wedge\tensor{e}{^{\mu_{D-1}}_{a_{D-1}}}\dd{x^{a_{D-1}}}\\
    \dd[D]{x}\sqrt{\abs{g}}&=\frac{1}{D!}\epsilon_{\mu_0\cdots\mu_{D-1}}\vb e^{\mu_0}\wedge\cdots\wedge\vb e^{\mu_{D-1}}
\end{align*}

And now we express the Ricci scalar,

\begin{align*}
    R&=g^{ab}\tensor{R}{_c_b^c_a}\\
    R&=\tensor{e}{_\rho^a}\tensor{e}{^\rho^b}\tensor{R}{_c_b_d_a}\tensor{e}{_\alpha^c}\tensor{e}{^\alpha^d}\\
    R&=\eta^{\rho\sigma}\eta^{\alpha\beta}\tensor{e}{_\rho^a}\tensor{e}{_\sigma^b}\tensor{R}{_c_b_d_a}\tensor{e}{_\alpha^c}\tensor{e}{_\beta^d}\\
    R&=\eta^{\rho\sigma}\eta^{\alpha\beta}\tensor{R}{_\alpha_\sigma_\beta_\rho}\\
    R&=\frac12\qty(\eta^{\rho\sigma}\eta^{\alpha\beta}-\eta^{\rho\alpha}\eta^{\sigma\beta})\tensor{R}{_\alpha_\sigma_\beta_\rho}\\
    R&=\frac{1}{2\qty(D-2)!}\tensor{\epsilon}{^{\nu_0}^\cdots^{\nu_{D-3}}^\beta^\rho}\tensor{\epsilon}{_{\nu_0}_\cdots_{\nu_{D-3}}^\alpha^\sigma}\tensor{R}{_\alpha_\sigma_\beta_\rho}
\end{align*}

Putting everything together,

\begin{align*}
    S_{\textnormal{EH}}&=\frac{1}{2\kappa}\int\limits_M\dd[D]{x}\sqrt{\abs{g}}R\\
    S_{\textnormal{EH}}&=\frac{1}{4D!\qty(D-2)!\kappa}\int\limits_M\vb e^{\mu_0}\wedge\cdots\wedge\vb e^{\mu_{D-1}}\epsilon_{\mu_0\cdots\mu_{D-1}}\tensor{\epsilon}{^{\nu_0}^\cdots^{\nu_{D-3}}^\beta^\rho}\tensor{\epsilon}{_{\nu_0}_\cdots_{\nu_{D-3}}^\alpha^\sigma}\tensor{R}{_\alpha_\sigma_\beta_\rho}\\
    S_{\textnormal{EH}}&=\frac{1}{4\qty(D-2)!\kappa}\int\limits_M\vb e^{\mu_0}\wedge\cdots\wedge\vb e^{\mu_{D-1}}\tensor{\eta}{_{\mu_0}^{[\nu_0}}\cdots\tensor{\eta}{_{\mu_{D-3}}^{\nu_{D-3}}}\tensor{\eta}{_{\mu_{D-2}}^{\beta}}\tensor{\eta}{_{\mu_{D-1}}^{\rho]}}\tensor{\epsilon}{_{\nu_0}_\cdots_{\nu_{D-3}}^\alpha^\sigma}\tensor{R}{_\alpha_\sigma_\beta_\rho}\\
    S_{\textnormal{EH}}&=\frac{1}{4\qty(D-2)!\kappa}\int\limits_M\vb e^{\nu_0}\wedge\cdots\wedge\vb e^{\nu_{D-3}}\wedge\vb e^{\beta}\wedge\vb e^{\rho}\tensor{\epsilon}{_{\nu_0}_\cdots_{\nu_{D-3}}^\alpha^\sigma}\tensor{R}{_\alpha_\sigma_\beta_\rho}\\
    S_{\textnormal{EH}}&=\frac{1}{2\kappa}\int\limits_M\frac{1}{2\qty(D-2)!}R_{\alpha\sigma\beta\rho}\tensor{\epsilon}{^\alpha^\sigma_{\nu_0}_\cdots_{\nu_{D-3}}}\vb e^{\nu_0}\wedge\cdots\wedge\vb e^{\nu_{D-3}}\wedge\vb e^{\beta}\wedge\vb e^{\rho}\\
    S_{\textnormal{EH}}&=\frac{1}{2\kappa}\int\limits_M\star\vb R_{\beta\rho}\wedge\vb e^{\beta}\wedge\vb e^{\rho}\\
    S_{\textnormal{EH}}&=\frac{1}{2\kappa}\int\limits_M\vb R_{\beta\rho}\wedge\star\qty(\vb e^{\beta}\wedge\vb e^{\rho})\\
    S_{\textnormal{EH}}&=\frac{1}{2\kappa}\int\limits_M\frac{1}{\qty(D-2)!}\tensor{\epsilon}{^\beta^\rho_{\alpha_0}_\cdots_{\alpha_{D-3}}}\vb R_{\beta\rho}\wedge\vb e^{\alpha_0}\wedge\cdots\wedge\vb e^{\alpha_{D-3}}\\
    S_{\textnormal{EH}}&=\frac{1}{2\qty(D-2)!\kappa}\int\limits_M\tensor{\epsilon}{_{\alpha_0}_\cdots_{\alpha_{D-1}}}\vb e^{\alpha_0}\wedge\cdots\wedge\vb e^{\alpha_{D-3}}\wedge\vb R^{\alpha_{D-2}\alpha_{D-1}}
\end{align*}

The most interesting case here is $D=3$,

\begin{align*}
    S_{\textnormal{EH}}\qty[\vb e,\boldsymbol\omega]&=\frac{1}{2\kappa}\epsilon_{\mu\alpha\beta}\int\limits_M\vb e^{\mu}\wedge\vb R^{\alpha\beta}
\end{align*}

Equations of motion are,

\begin{align*}
    S_{\textnormal{EH}}\qty[\vb e+\delta\vb e,\boldsymbol\omega]-S_{\textnormal{EH}}\qty[\vb e,\boldsymbol\omega]&=\frac{1}{2\kappa}\epsilon_{\mu\alpha\beta}\int\limits_M\delta\vb e^{\mu}\wedge\vb R^{\alpha\beta}=0\\
    0&=-\frac12\epsilon_{\mu\alpha\beta}\vb R^{\alpha\beta}\\
    0&=-\frac12\epsilon_{\mu\alpha\beta}\frac12\tensor{R}{_\rho_\sigma^\alpha^\beta}\vb e^\rho\wedge\vb e^\sigma\\
    0&=-\frac14\epsilon_{\mu\alpha\beta}\tensor{R}{_\rho_\sigma^\alpha^\beta}\star\qty(\vb e^\rho\wedge\vb e^\sigma)\\
    0&=-\frac14\epsilon_{\mu\alpha\beta}\tensor{R}{_\rho_\sigma^\alpha^\beta}\tensor{\epsilon}{^\rho^\sigma_\kappa}\vb e^\kappa\\
    0&=-\frac14\epsilon_{\mu\alpha\beta}\tensor{\epsilon}{^\rho^\sigma^\kappa}\tensor{R}{_\rho_\sigma^\alpha^\beta}\vb e_\kappa\\
    0&=-\frac14\tensor{\eta}{_\mu^{[\rho}}\tensor{\eta}{_\alpha^{\sigma}}\tensor{\eta}{_\beta^{\kappa]}}\tensor{R}{_\rho_\sigma^\alpha^\beta}\vb e_\kappa\\
    0&=-\frac14\tensor{R}{_\rho_\sigma^{[\sigma}^\kappa}\tensor{\eta}{_\mu^{\rho]}}\vb e_\kappa\\
    0&=-\frac14\qty(\tensor{R}{_\rho_\sigma^{\sigma}^\kappa}\tensor{\eta}{_\mu^{\rho}}+\tensor{R}{_\rho_\sigma^\kappa^\rho}\tensor{\eta}{_\mu^{\sigma}}+\tensor{R}{_\rho_\sigma^\rho^\sigma}\tensor{\eta}{_\mu^\kappa}-\tensor{R}{_\rho_\sigma^{\rho}^\kappa}\tensor{\eta}{_\mu^{\sigma}}-\tensor{R}{_\rho_\sigma^\kappa^\sigma}\tensor{\eta}{_\mu^{\rho}}-\tensor{R}{_\rho_\sigma^\sigma^\rho}\tensor{\eta}{_\mu^\kappa})\vb e_\kappa\\
    0&=-\frac14\qty(-\tensor{R}{_\mu^\kappa}-\tensor{R}{_\mu^\kappa}+R\tensor{\eta}{_\mu^\kappa}-\tensor{R}{_\mu^\kappa}-\tensor{R}{_\mu^\kappa}+R\tensor{\eta}{_\mu^\kappa})\vb e_\kappa\\
    0&=-\frac14(-4\tensor{R}{_\mu^\kappa}+2R\tensor{\eta}{_\mu^\kappa})\vb e_\kappa\\
    0&=\qty(\tensor{R}{_\mu_\kappa}-\frac12R\tensor{\eta}{_\mu_\kappa})\vb e^\kappa
\end{align*}

And,

\begin{align*}
    S_{\textnormal{EH}}\qty[\vb e,\boldsymbol\omega+\delta\boldsymbol\omega]-S_{\textnormal{EH}}\qty[\vb e,\boldsymbol\omega]&=\frac{1}{2\kappa}\epsilon_{\mu\alpha\beta}\int\limits_M\vb e^{\mu}\wedge\qty(\dd{\delta\boldsymbol\omega}+\delta\boldsymbol\omega\wedge\boldsymbol\omega+\boldsymbol\omega\wedge\delta\boldsymbol\omega)^{\alpha\beta}=0\\
    0&=\frac{1}{2\kappa}\epsilon_{\mu\alpha\beta}\int\limits_M\qty(-\dd{\qty(\vb e^\mu\wedge\delta\boldsymbol\omega^{\alpha\beta})}+\dd{\vb e^\mu}\wedge\delta\boldsymbol\omega^{\alpha\beta}+\vb e^\mu\wedge\qty(\delta\boldsymbol\omega\wedge\boldsymbol\omega)^{\alpha\beta}+\vb e^\mu\wedge\qty(\boldsymbol\omega\wedge\delta\boldsymbol\omega)^{\alpha\beta})\\
    0&=\frac{1}{2}\epsilon_{\mu\alpha\beta}\int\limits_M\qty(\dd{\vb e^\mu}\wedge\delta\boldsymbol\omega^{\alpha\beta}+\vb e^\mu\wedge\tensor{\delta\boldsymbol\omega}{^\alpha^\gamma}\wedge\tensor{\boldsymbol\omega}{_\gamma^\beta}+\vb e^\mu\wedge\tensor{\boldsymbol\omega}{^\alpha^\gamma}\wedge\tensor{\delta\boldsymbol\omega}{_\gamma^\beta})\\
    0&=\frac{1}{2}\epsilon_{\mu\alpha\beta}\int\limits_M\qty(\dd{\vb e^\mu}\wedge\delta\boldsymbol\omega^{\alpha\beta}-\vb e^\mu\wedge\tensor{\boldsymbol\omega}{_\gamma^\beta}\wedge\tensor{\delta\boldsymbol\omega}{^\alpha^\gamma}+\vb e^\mu\wedge\tensor{\boldsymbol\omega}{^\alpha_\gamma}\wedge\tensor{\delta\boldsymbol\omega}{^\gamma^\beta})\\
    0&=\frac{1}{2}\epsilon_{\mu\alpha\beta}\int\limits_M\dd{\vb e^\mu}\wedge\delta\boldsymbol\omega^{\alpha\beta}-\frac{1}{2}\epsilon_{\mu\alpha\beta}\vb e^\mu\wedge\tensor{\boldsymbol\omega}{_\gamma^\beta}\wedge\tensor{\delta\boldsymbol\omega}{^\alpha^\gamma}+\frac{1}{2}\epsilon_{\mu\alpha\beta}\vb e^\mu\wedge\tensor{\boldsymbol\omega}{^\alpha_\gamma}\wedge\tensor{\delta\boldsymbol\omega}{^\gamma^\beta}\\
    0&=\frac{1}{2}\epsilon_{\mu\alpha\beta}\int\limits_M\dd{\vb e^\mu}\wedge\delta\boldsymbol\omega^{\alpha\beta}-\frac{1}{2}\epsilon_{\mu\alpha\gamma}\vb e^\mu\wedge\tensor{\boldsymbol\omega}{_\beta^\gamma}\wedge\tensor{\delta\boldsymbol\omega}{^\alpha^\beta}+\frac{1}{2}\epsilon_{\mu\gamma\beta}\vb e^\mu\wedge\tensor{\boldsymbol\omega}{^\gamma_\alpha}\wedge\tensor{\delta\boldsymbol\omega}{^\alpha^\beta}\\
    0&=\frac{1}{2}\int\limits_M\qty(\epsilon_{\mu\alpha\beta}\dd{\vb e^\mu}-\epsilon_{\mu\alpha\gamma}\vb e^\mu\wedge\tensor{\boldsymbol\omega}{_\beta^\gamma}+\epsilon_{\mu\gamma\beta}\vb e^\mu\wedge\tensor{\boldsymbol\omega}{^\gamma_\alpha})\wedge\tensor{\delta\boldsymbol\omega}{^\alpha^\beta}\\
    0&=\frac{1}{2}\epsilon_{\mu\alpha\beta}\dd{\vb e^\mu}-\frac{1}{2}\epsilon_{\mu\alpha\gamma}\vb e^\mu\wedge\tensor{\boldsymbol\omega}{_\beta^\gamma}+\frac{1}{2}\epsilon_{\mu\gamma\beta}\vb e^\mu\wedge\tensor{\boldsymbol\omega}{^\gamma_\alpha}\\
    0&=\frac{1}{2}\epsilon^{\alpha\beta\nu}\epsilon_{\mu\alpha\beta}\dd{\vb e^\mu}-\frac{1}{2}\epsilon^{\alpha\beta\nu}\epsilon_{\mu\alpha\gamma}\vb e^\mu\wedge\tensor{\boldsymbol\omega}{_\beta^\gamma}+\frac{1}{2}\epsilon^{\alpha\beta\nu}\epsilon_{\mu\gamma\beta}\vb e^\mu\wedge\tensor{\boldsymbol\omega}{^\gamma_\alpha}\\
    0&=\dd{\vb e^\nu}-\tensor{\eta}{_\gamma^{[\beta}}\tensor{\eta}{_\mu^{\nu]}}\vb e^\mu\wedge\tensor{\boldsymbol\omega}{_\beta^\gamma}+\tensor{\eta}{_\mu^{[\nu}}\tensor{\eta}{_\gamma^{\alpha]}}\vb e^\mu\wedge\tensor{\boldsymbol\omega}{^\gamma_\alpha}\\
    0&=\dd{\vb e^\nu}-\frac{1}{2}\qty(\tensor{\eta}{_\gamma^{\beta}}\tensor{\eta}{_\mu^{\nu}}-\tensor{\eta}{_\gamma^{\nu}}\tensor{\eta}{_\mu^{\beta}})\vb e^\mu\wedge\tensor{\boldsymbol\omega}{_\beta^\gamma}+\frac{1}{2}\qty(\tensor{\eta}{_\mu^{\nu}}\tensor{\eta}{_\gamma^{\alpha}}-\tensor{\eta}{_\mu^{\alpha}}\tensor{\eta}{_\gamma^{\nu}})\vb e^\mu\wedge\tensor{\boldsymbol\omega}{^\gamma_\alpha}\\
    0&=\dd{\vb e^\nu}+\frac{1}{2}\tensor{\eta}{_\gamma^{\nu}}\tensor{\eta}{_\mu^{\beta}}\vb e^\mu\wedge\tensor{\boldsymbol\omega}{_\beta^\gamma}-\frac{1}{2}\tensor{\eta}{_\mu^{\alpha}}\tensor{\eta}{_\gamma^{\nu}}\vb e^\mu\wedge\tensor{\boldsymbol\omega}{^\gamma_\alpha}\\
    0&=\dd{\vb e^\nu}+\frac{1}{2}\vb e^\beta\wedge\tensor{\boldsymbol\omega}{_\beta^\nu}-\frac{1}{2}\vb e^\alpha\wedge\tensor{\boldsymbol\omega}{^\nu_\alpha}\\
    0&=\dd{\vb e^\nu}+\tensor{\boldsymbol\omega}{^\nu_\alpha}\wedge\vb e^\alpha
\end{align*}

It's not really feasible to give this a gauge theory approach, only if we're in 2+1, in this case there is an isomorphism, $\vb e^\mu\rightarrow \vb e_{\alpha\beta}=\epsilon_{\mu\alpha\beta}\vb e^\mu$, so that,

\begin{align*}
    S_{\textnormal{EH}}&=\frac{1}{2\kappa}\epsilon_{\mu\alpha\beta}\int\limits_M\vb e^\mu\wedge \vb R^{\alpha\beta}\\
    S_{\textnormal{EH}}&=-\frac{1}{2\kappa}\int\limits_M\vb e_{\beta\alpha}\wedge \vb R^{\alpha\beta}\\
    S_{\textnormal{EH}}&=-\frac{1}{2\kappa}\int\limits_M\Tr\qty[\vb e\wedge \vb R]\\
    S_{\textnormal{EH}}&=-\frac{1}{2\kappa}\int\limits_M\Tr\qty[\vb e\wedge\qty(\dd{\boldsymbol\omega}+\frac12\wedgecomm{\boldsymbol\omega}{\boldsymbol\omega})]
\end{align*}

This is a lot similar to Chern-Simons theory,

\begin{align*}
    S_{\textnormal{CS}}\qty[\vb A]&=k\int\limits_M\Tr\qty[\vb A\wedge\dd{\vb A}+\frac13\vb A\wedge\wedgecomm{\vb A}{\vb A}]
\end{align*}

Let's try, $\vb A^x=\boldsymbol\omega+x\vb e$,

\begin{align*}
    S_{\textnormal{CS}}\qty[\vb A^x]&=k\int\limits_M\Tr\qty[\qty(\boldsymbol\omega+x\vb e)\wedge\dd{\qty(\boldsymbol\omega+x\vb e)}+\frac13\qty(\boldsymbol\omega+x\vb e)\wedge\wedgecomm{\boldsymbol\omega+x\vb e}{\boldsymbol\omega+x\vb e}]\\
    S_{\textnormal{CS}}\qty[\vb A^x]&=k\int\limits_M\Tr\biggl[\boldsymbol\omega\wedge\dd{\boldsymbol\omega}+x\boldsymbol\omega\wedge\dd{\vb e}+x\vb e\wedge\dd{\boldsymbol\omega}+x^2\vb e\wedge\dd{\vb e}\\
    &\quad\quad\quad\left.+\frac23\qty(\boldsymbol\omega+x\vb e)\wedge\qty(\boldsymbol\omega+x\vb e)\wedge\qty(\boldsymbol\omega+x\vb e)\right]\\
    S_{\textnormal{CS}}\qty[\vb A^x]&=k\int\limits_M\Tr\biggl[\boldsymbol\omega\wedge\dd{\boldsymbol\omega}+x\dd{\vb e}\wedge\boldsymbol\omega+x\vb e\wedge\dd{\boldsymbol\omega}-\frac12x^2\dd{\qty(\vb e\wedge\vb e)}\\
    &\quad\quad\quad\left.+\frac23\boldsymbol\omega\wedge\boldsymbol\omega\wedge\boldsymbol\omega+2x\boldsymbol\omega\wedge\boldsymbol\omega\wedge\vb e+2x^2\vb e\wedge\vb e\wedge \boldsymbol\omega+\frac23x^3\vb e\wedge\vb e\wedge\vb e\right]\\
    S_{\textnormal{CS}}\qty[\vb A^x]&=k\int\limits_M\Tr\left[\boldsymbol\omega\wedge\qty(\dd{\boldsymbol\omega}+\frac23\boldsymbol\omega\wedge\boldsymbol\omega)+x\dd{\qty(\vb e\wedge\boldsymbol\omega)}+x\vb e\wedge\dd{\boldsymbol\omega}+x\vb e\wedge\qty(\dd{\boldsymbol\omega}+2\boldsymbol\omega\wedge\boldsymbol\omega)+2x^2\vb e\wedge\boldsymbol\omega\wedge\vb e\right.\\
    &\quad\quad\quad\left.+\frac23x^3\vb e\wedge\vb e\wedge\vb e\right]\\
    S_{\textnormal{CS}}\qty[\vb A^x]&=S_{\textnormal{CS}}\qty[\boldsymbol\omega]+k\int\limits_M\Tr\qty[x\dd{\qty(\vb e\wedge\boldsymbol\omega)}+2x\vb e\wedge\qty(\dd{\boldsymbol\omega}+\boldsymbol\omega\wedge\boldsymbol\omega)+2x^2\vb e\wedge\boldsymbol\omega\wedge\vb e+\frac23x^3\vb e\wedge\vb e\wedge\vb e]\\
    S_{\textnormal{CS}}\qty[\vb A^x]&=S_{\textnormal{CS}}\qty[\boldsymbol\omega]+k\int\limits_M\Tr\qty[x\dd{\qty(\vb e\wedge\boldsymbol\omega)}+2x\vb e\wedge\vb R+2x^2\vb e\wedge\boldsymbol\omega\wedge\vb e+\frac23x^3\vb e\wedge\vb e\wedge\vb e]\\
    S_{\textnormal{CS}}\qty[\vb A^x]&=S_{\textnormal{CS}}\qty[\boldsymbol\omega]-4xk\kappa S_{\textnormal{EH}}+k\int\limits_M\Tr\qty[x\dd{\qty(\vb e\wedge\boldsymbol\omega)}+2x^2\vb e\wedge\boldsymbol\omega\wedge\vb e+\frac23x^3\vb e\wedge\vb e\wedge\vb e]
\end{align*}

We can simplify if we sum two contributions,

\begin{align*}
    S_{\textnormal{CS}}\qty[\vb A^x]-S_{\textnormal{CS}}\qty[\vb A^{-x}]&=-8xk\kappa S_{\textnormal{EH}}+2kx\int\limits_{\partial M}\Tr\qty[\vb e\wedge\boldsymbol\omega]+\frac43x^3k\int\limits_M\Tr\qty[\vb e\wedge\vb e\wedge\vb e]\\
    \frac{1}{8xk\kappa}\qty(S_{\textnormal{CS}}\qty[\vb A^{-x}]-S_{\textnormal{CS}}\qty[\vb A^x])&=S_{\textnormal{EH}}-\frac{1}{4\kappa}\int\limits_{\partial M}\Tr\qty[\vb e\wedge\boldsymbol\omega]-\frac{x^2}{3!\kappa}\int\limits_M\Tr\qty[\vb e\wedge\vb e\wedge\vb e]
\end{align*}

And also the not so usual action,

\begin{align*}
    S_{\textnormal{CS}}\qty[\vb A^x]+S_{\textnormal{CS}}\qty[\vb A^{-x}]&=2S_{\textnormal{CS}}\qty[\boldsymbol\omega]+4x^2k\int\limits_M\Tr\qty[\vb e\wedge\boldsymbol\omega\wedge\vb e]
\end{align*}

Chern-Simons Equation of Motion,

\begin{align*}
    S_{\textnormal{CS}}\qty[\vb A+\delta\vb A]-S_{\textnormal{CS}}\qty[\vb A]&=k\int\limits_M\Tr\qty[\delta\vb A\wedge\dd{\vb A}+\vb A\wedge\dd{\delta\vb A}+\frac23\delta\vb A\wedge\vb A\wedge\vb A+\frac23\vb A\wedge\delta\vb A\wedge\vb A+\frac23\vb A\wedge\vb A\wedge\delta\vb A]\\
    S_{\textnormal{CS}}\qty[\vb A+\delta\vb A]-S_{\textnormal{CS}}\qty[\vb A]&=k\int\limits_M\Tr\qty[\dd{\vb A}\wedge\delta\vb A-\dd{\qty(\vb A\wedge\delta\vb A)}+\dd{\vb A}\wedge\delta \vb A+2\vb A\wedge\vb A\wedge\delta\vb A]\\
    S_{\textnormal{CS}}\qty[\vb A+\delta\vb A]-S_{\textnormal{CS}}\qty[\vb A]&=2k\int\limits_M\Tr\qty[\qty(\dd{\vb A}+\vb A\wedge\vb A)\wedge\delta\vb A]-k\int\limits_M\Tr\qty[\dd{\qty(\vb A\wedge\delta\vb A)}]\\
    S_{\textnormal{CS}}\qty[\vb A+\delta\vb A]-S_{\textnormal{CS}}\qty[\vb A]&=2k\int\limits_M\Tr\qty[\vb F\wedge\delta\vb A]-k\int\limits_{\partial M}\Tr\qty[\vb A\wedge\delta\vb A]
\end{align*}