\section{Gravity as a Gauge Theory}

Let's take a step backwards to breath, this last expression was our goal to reach, it shows the Einstein-Hilbert Action\footnote{Actually it's the Einstein-Cartan Action, as we have not imposed the torsionless condition, but, we'll not bother distinguishing this.} 
written exactly in term of the vielbein and the spin connection 1--forms, in particular, the spin connection as being the connection form of the gauged Lorentz transformations shows up only inside the curvature 2--form, as 
it should happen to a gauge theory, this guarantees the manifestly local Lorentz invariance, to see this, we defined the local Lorentz redundancy as being $\tilde{\vb e}_\mu\rightarrow \tensor{\Lambda}{^\nu_\mu}\tilde{\vb e}_\nu$, with the corresponding 
transformation on $\boldsymbol\omega$ derived before, but, the vector vielbein transformation actually induces a transformation in the covector vielbein by, $\vb e^\mu\qty(\tilde{\vb e}_\nu)=\tensor{\delta}{^\mu_\nu}\Rightarrow \vb e^\mu\rightarrow \tensor{\Lambda}{^{-1}^\mu_\nu}\vb e^\nu$, so that the 
relevant expressions for us now are\footnote{For convenience we'll make the change $\Lambda\leftrightarrow\Lambda^{-1}$ everywhere.},
\begin{align*}
    \begin{cases}
        \vb e^\mu&\rightarrow\tensor{\Lambda}{^\mu_\nu}\vb e^\nu\\
        \tensor{\boldsymbol\omega}{^\alpha_\beta}&\rightarrow\tensor{\Lambda}{^\alpha_\rho}\tensor{\boldsymbol\omega}{^\rho_\sigma}\tensor{\Lambda}{^{-1}^\sigma_\beta}+\tensor{\Lambda}{^\alpha_\sigma}\vb d\tensor{\Lambda}{^{-1}^\sigma_\beta}
    \end{cases}\Leftrightarrow\begin{cases}
        \vb e&\rightarrow\Lambda\vb e\\
        \boldsymbol\omega&\rightarrow\Lambda\boldsymbol\omega\Lambda^{-1}+\Lambda\vb d\Lambda^{-1}
    \end{cases} 
\end{align*}
where we also included the matrix form of these transformations, to see the invariance of the action with respect to these is only needed to work out the transformation law of the curvature 2--form,
\begin{align*}
    \vb R&=\vb d\boldsymbol\omega+\boldsymbol\omega\wedge\boldsymbol\omega\rightarrow \vb d\qty(\Lambda\boldsymbol\omega\Lambda^{-1}+\Lambda\vb d\Lambda^{-1})+\qty(\Lambda\boldsymbol\omega\Lambda^{-1}+\Lambda\vb d\Lambda^{-1})\wedge\qty(\Lambda\boldsymbol\omega\Lambda^{-1}+\Lambda\vb d\Lambda^{-1})\\
    \vb R&\rightarrow \vb d\Lambda\wedge\boldsymbol\omega\Lambda^{-1}+\Lambda\vb d\boldsymbol\omega\Lambda^{-1}-\Lambda\boldsymbol\omega\wedge\vb d\Lambda^{-1}+\vb d\Lambda\wedge\vb d\Lambda^{-1}+\Lambda\boldsymbol\omega\wedge\boldsymbol\omega\Lambda^{-1}+\Lambda\boldsymbol\omega\wedge\vb d\Lambda^{-1}-\vb d\Lambda\wedge\boldsymbol\omega\Lambda^{-1}-\vb d\Lambda\wedge\vb d\Lambda^{-1}\\
    \vb R&\rightarrow \Lambda\qty(\vb d\boldsymbol\omega+\boldsymbol\omega\wedge\boldsymbol\omega)\Lambda^{-1}=\Lambda\vb R\Lambda^{-1}
\end{align*}
and lastly, but not less important, we have to understand whether or not the Hodge star operator should change or not with respect to this transformation, the answer is no\footnote{As long as we work with orientation preserving transformation, otherwise it'll adquire an extra sign.}, despite it depending explicitly on the 
metric to be defined, it's dependence is only through $\sqrt{\abs{\Det\qty[g_{ab}]}}$, which is invariant under a local Lorentz transformation, as $g_{ab}=\eta_{\mu\nu}\tensor{e}{^\mu_a}\tensor{e}{^\nu_b}$, thus, $\star\vb R\rightarrow \Lambda\qty(\star\vb R)\Lambda^{-1}$, and the action is manifestly invariant,
\begin{align*}
    S_{\textnormal{EH}}'=\frac{1}{2\kappa}\int\limits_M\tensor{\Lambda}{_\beta^\tau}\star\vb R_{\tau\sigma}\tensor{\Lambda}{^{-1}^\sigma_\rho}\wedge\tensor{\Lambda}{^\beta_\alpha}\vb e^\alpha\wedge\tensor{\Lambda}{^\rho_\mu}\vb e^\mu=\frac{1}{2\kappa}\int\limits_M\star\vb R_{\beta\rho}\wedge\vb e^{\beta}\wedge\vb e^{\rho}=S_{\textnormal{EH}}
\end{align*}





\begin{align*}
    S_{\textnormal{EH}}&=\frac{1}{2\kappa}\int\limits_M\vb R_{\beta\rho}\wedge\star\qty(\vb e^{\beta}\wedge\vb e^{\rho})\\
    S_{\textnormal{EH}}&=\frac{1}{2\kappa}\int\limits_M\frac{1}{\qty(D-2)!}\tensor{\epsilon}{^\beta^\rho_{\alpha_1}_\cdots_{\alpha_{D-2}}}\vb R_{\beta\rho}\wedge\vb e^{\alpha_1}\wedge\cdots\wedge\vb e^{\alpha_{D-2}}\\
    S_{\textnormal{EH}}&=\frac{1}{2\qty(D-2)!\kappa}\int\limits_M\tensor{\epsilon}{_{\alpha_1}_\cdots_{\alpha_{D}}}\vb e^{\alpha_1}\wedge\cdots\wedge\vb e^{\alpha_{D-2}}\wedge\vb R^{\alpha_{D-1}\alpha_{D}}
\end{align*}

For $D=4$ this gives,
\begin{align*}
    S_{\textnormal{EH}}\qty[\vb e,\boldsymbol\omega]&=\frac{1}{4\kappa}\epsilon_{\mu\nu\alpha\beta}\int\limits_M\vb e^{\mu}\wedge\vb e^\nu\wedge\vb R^{\alpha\beta}
\end{align*}

It's not clear how this should be interpreted as a gauge theory, due to we wanting to interpret $\boldsymbol\omega$ as the gauge 1-form of Lorentz transformations and $\tilde{\vb e}$ as the gauge 1-form of 
translations, the Einstein Hilbert Action should then be something of the form,
\begin{align*}
    \int\limits_M\Tr\qty[\vb A\wedge\vb A\wedge\vb F]
\end{align*}
for a combined gauge field $\vb A$, where both $\boldsymbol\omega$ and $\vb e$ contribute in some way, sadly, there is no such gauge theory in this form, 
first, due to the trace being of three lie algebra valued forms, this vanishes, secondly, this is not invariant under a gauge transformation $\vb A\rightarrow g^{-1}\vb Ag+g^{-1}\dd{g}$. So, 
if it's to $3+1$ gravity to be a gauge theory in this sense, it certainly is realized in a different way, but, an interesting case happens to $D=2+1$,
\begin{align*}
    S_{\textnormal{EH}}\qty[\vb e,\boldsymbol\omega]&=\frac{1}{2\kappa}\epsilon_{\mu\alpha\beta}\int\limits_M\vb e^{\mu}\wedge\vb R^{\alpha\beta}
\end{align*}

This already seems a lot like a proper gauge theory of the Chern-Simons type,
Equations of motion are,
\begin{align*}
    S_{\textnormal{EH}}\qty[\vb e+\delta\vb e,\boldsymbol\omega]-S_{\textnormal{EH}}\qty[\vb e,\boldsymbol\omega]&=\frac{1}{2\kappa}\epsilon_{\mu\alpha\beta}\int\limits_M\delta\vb e^{\mu}\wedge\vb R^{\alpha\beta}=0\\
    0&=-\frac12\epsilon_{\mu\alpha\beta}\vb R^{\alpha\beta}\\
    0&=-\frac12\epsilon_{\mu\alpha\beta}\frac12\tensor{R}{_\rho_\sigma^\alpha^\beta}\vb e^\rho\wedge\vb e^\sigma\\
    0&=-\frac14\epsilon_{\mu\alpha\beta}\tensor{R}{_\rho_\sigma^\alpha^\beta}\star\qty(\vb e^\rho\wedge\vb e^\sigma)\\
    0&=-\frac14\epsilon_{\mu\alpha\beta}\tensor{R}{_\rho_\sigma^\alpha^\beta}\tensor{\epsilon}{^\rho^\sigma_\kappa}\vb e^\kappa\\
    0&=-\frac14\epsilon_{\mu\alpha\beta}\tensor{\epsilon}{^\rho^\sigma^\kappa}\tensor{R}{_\rho_\sigma^\alpha^\beta}\vb e_\kappa\\
    0&=-\frac{3!}{4}\tensor{\eta}{_\mu^{[\rho}}\tensor{\eta}{_\alpha^{\sigma}}\tensor{\eta}{_\beta^{\kappa]}}\tensor{R}{_\rho_\sigma^\alpha^\beta}\vb e_\kappa\\
    0&=-\frac{3!}{4}\tensor{R}{_\rho_\sigma^{[\sigma}^\kappa}\tensor{\eta}{_\mu^{\rho]}}\vb e_\kappa\\
    0&=-\frac14\qty(\tensor{R}{_\rho_\sigma^{\sigma}^\kappa}\tensor{\eta}{_\mu^{\rho}}+\tensor{R}{_\rho_\sigma^\kappa^\rho}\tensor{\eta}{_\mu^{\sigma}}+\tensor{R}{_\rho_\sigma^\rho^\sigma}\tensor{\eta}{_\mu^\kappa}-\tensor{R}{_\rho_\sigma^{\rho}^\kappa}\tensor{\eta}{_\mu^{\sigma}}-\tensor{R}{_\rho_\sigma^\kappa^\sigma}\tensor{\eta}{_\mu^{\rho}}-\tensor{R}{_\rho_\sigma^\sigma^\rho}\tensor{\eta}{_\mu^\kappa})\vb e_\kappa\\
    0&=-\frac14\qty(-\tensor{R}{_\mu^\kappa}-\tensor{R}{_\mu^\kappa}+R\tensor{\eta}{_\mu^\kappa}-\tensor{R}{_\mu^\kappa}-\tensor{R}{_\mu^\kappa}+R\tensor{\eta}{_\mu^\kappa})\vb e_\kappa\\
    0&=-\frac14(-4\tensor{R}{_\mu^\kappa}+2R\tensor{\eta}{_\mu^\kappa})\vb e_\kappa\\
    0&=\qty(\tensor{R}{_\mu_\kappa}-\frac12R\tensor{\eta}{_\mu_\kappa})\vb e^\kappa
\end{align*}

And,
\begin{align*}
    S_{\textnormal{EH}}\qty[\vb e,\boldsymbol\omega+\delta\boldsymbol\omega]-S_{\textnormal{EH}}\qty[\vb e,\boldsymbol\omega]&=\frac{1}{2\kappa}\epsilon_{\mu\alpha\beta}\int\limits_M\vb e^{\mu}\wedge\qty(\dd{\delta\boldsymbol\omega}+\delta\boldsymbol\omega\wedge\boldsymbol\omega+\boldsymbol\omega\wedge\delta\boldsymbol\omega)^{\alpha\beta}=0\\
    0&=\frac{1}{2\kappa}\epsilon_{\mu\alpha\beta}\int\limits_M\qty(-\dd{\qty(\vb e^\mu\wedge\delta\boldsymbol\omega^{\alpha\beta})}+\dd{\vb e^\mu}\wedge\delta\boldsymbol\omega^{\alpha\beta}+\vb e^\mu\wedge\qty(\delta\boldsymbol\omega\wedge\boldsymbol\omega)^{\alpha\beta}+\vb e^\mu\wedge\qty(\boldsymbol\omega\wedge\delta\boldsymbol\omega)^{\alpha\beta})\\
    0&=\frac{1}{2}\epsilon_{\mu\alpha\beta}\int\limits_M\qty(\dd{\vb e^\mu}\wedge\delta\boldsymbol\omega^{\alpha\beta}+\vb e^\mu\wedge\tensor{\delta\boldsymbol\omega}{^\alpha^\gamma}\wedge\tensor{\boldsymbol\omega}{_\gamma^\beta}+\vb e^\mu\wedge\tensor{\boldsymbol\omega}{^\alpha^\gamma}\wedge\tensor{\delta\boldsymbol\omega}{_\gamma^\beta})\\
    0&=\frac{1}{2}\epsilon_{\mu\alpha\beta}\int\limits_M\qty(\dd{\vb e^\mu}\wedge\delta\boldsymbol\omega^{\alpha\beta}-\vb e^\mu\wedge\tensor{\boldsymbol\omega}{_\gamma^\beta}\wedge\tensor{\delta\boldsymbol\omega}{^\alpha^\gamma}+\vb e^\mu\wedge\tensor{\boldsymbol\omega}{^\alpha_\gamma}\wedge\tensor{\delta\boldsymbol\omega}{^\gamma^\beta})\\
    0&=\frac{1}{2}\epsilon_{\mu\alpha\beta}\int\limits_M\dd{\vb e^\mu}\wedge\delta\boldsymbol\omega^{\alpha\beta}-\frac{1}{2}\epsilon_{\mu\alpha\beta}\vb e^\mu\wedge\tensor{\boldsymbol\omega}{_\gamma^\beta}\wedge\tensor{\delta\boldsymbol\omega}{^\alpha^\gamma}+\frac{1}{2}\epsilon_{\mu\alpha\beta}\vb e^\mu\wedge\tensor{\boldsymbol\omega}{^\alpha_\gamma}\wedge\tensor{\delta\boldsymbol\omega}{^\gamma^\beta}\\
    0&=\frac{1}{2}\epsilon_{\mu\alpha\beta}\int\limits_M\dd{\vb e^\mu}\wedge\delta\boldsymbol\omega^{\alpha\beta}-\frac{1}{2}\epsilon_{\mu\alpha\gamma}\vb e^\mu\wedge\tensor{\boldsymbol\omega}{_\beta^\gamma}\wedge\tensor{\delta\boldsymbol\omega}{^\alpha^\beta}+\frac{1}{2}\epsilon_{\mu\gamma\beta}\vb e^\mu\wedge\tensor{\boldsymbol\omega}{^\gamma_\alpha}\wedge\tensor{\delta\boldsymbol\omega}{^\alpha^\beta}\\
    0&=\frac{1}{2}\int\limits_M\qty(\epsilon_{\mu\alpha\beta}\dd{\vb e^\mu}-\epsilon_{\mu\alpha\gamma}\vb e^\mu\wedge\tensor{\boldsymbol\omega}{_\beta^\gamma}+\epsilon_{\mu\gamma\beta}\vb e^\mu\wedge\tensor{\boldsymbol\omega}{^\gamma_\alpha})\wedge\tensor{\delta\boldsymbol\omega}{^\alpha^\beta}\\
    0&=\frac{1}{2}\epsilon_{\mu\alpha\beta}\dd{\vb e^\mu}-\frac{1}{2}\epsilon_{\mu\alpha\gamma}\vb e^\mu\wedge\tensor{\boldsymbol\omega}{_\beta^\gamma}+\frac{1}{2}\epsilon_{\mu\gamma\beta}\vb e^\mu\wedge\tensor{\boldsymbol\omega}{^\gamma_\alpha}\\
    0&=\frac{1}{2}\epsilon^{\alpha\beta\nu}\epsilon_{\mu\alpha\beta}\dd{\vb e^\mu}-\frac{1}{2}\epsilon^{\alpha\beta\nu}\epsilon_{\mu\alpha\gamma}\vb e^\mu\wedge\tensor{\boldsymbol\omega}{_\beta^\gamma}+\frac{1}{2}\epsilon^{\alpha\beta\nu}\epsilon_{\mu\gamma\beta}\vb e^\mu\wedge\tensor{\boldsymbol\omega}{^\gamma_\alpha}\\
    0&=\dd{\vb e^\nu}-\tensor{\eta}{_\gamma^{[\beta}}\tensor{\eta}{_\mu^{\nu]}}\vb e^\mu\wedge\tensor{\boldsymbol\omega}{_\beta^\gamma}+\tensor{\eta}{_\mu^{[\nu}}\tensor{\eta}{_\gamma^{\alpha]}}\vb e^\mu\wedge\tensor{\boldsymbol\omega}{^\gamma_\alpha}\\
    0&=\dd{\vb e^\nu}-\frac{1}{2}\qty(\tensor{\eta}{_\gamma^{\beta}}\tensor{\eta}{_\mu^{\nu}}-\tensor{\eta}{_\gamma^{\nu}}\tensor{\eta}{_\mu^{\beta}})\vb e^\mu\wedge\tensor{\boldsymbol\omega}{_\beta^\gamma}+\frac{1}{2}\qty(\tensor{\eta}{_\mu^{\nu}}\tensor{\eta}{_\gamma^{\alpha}}-\tensor{\eta}{_\mu^{\alpha}}\tensor{\eta}{_\gamma^{\nu}})\vb e^\mu\wedge\tensor{\boldsymbol\omega}{^\gamma_\alpha}\\
    0&=\dd{\vb e^\nu}+\frac{1}{2}\tensor{\eta}{_\gamma^{\nu}}\tensor{\eta}{_\mu^{\beta}}\vb e^\mu\wedge\tensor{\boldsymbol\omega}{_\beta^\gamma}-\frac{1}{2}\tensor{\eta}{_\mu^{\alpha}}\tensor{\eta}{_\gamma^{\nu}}\vb e^\mu\wedge\tensor{\boldsymbol\omega}{^\gamma_\alpha}\\
    0&=\dd{\vb e^\nu}+\frac{1}{2}\vb e^\beta\wedge\tensor{\boldsymbol\omega}{_\beta^\nu}-\frac{1}{2}\vb e^\alpha\wedge\tensor{\boldsymbol\omega}{^\nu_\alpha}\\
    0&=\dd{\vb e^\nu}+\tensor{\boldsymbol\omega}{^\nu_\alpha}\wedge\vb e^\alpha
\end{align*}

It's not really feasible to give this a gauge theory approach, only if we're in 2+1, in this case there is an isomorphism, $\vb e^\mu\rightarrow \vb e_{\alpha\beta}=\epsilon_{\mu\alpha\beta}\vb e^\mu$, so that,
\begin{align*}
    S_{\textnormal{EH}}&=\frac{1}{2\kappa}\epsilon_{\mu\alpha\beta}\int\limits_M\vb e^\mu\wedge \vb R^{\alpha\beta}\\
    S_{\textnormal{EH}}&=-\frac{1}{2\kappa}\int\limits_M\vb e_{\beta\alpha}\wedge \vb R^{\alpha\beta}\\
    S_{\textnormal{EH}}&=-\frac{1}{2\kappa}\int\limits_M\Tr\qty[\vb e\wedge \vb R]\\
    S_{\textnormal{EH}}&=-\frac{1}{2\kappa}\int\limits_M\Tr\qty[\vb e\wedge\qty(\dd{\boldsymbol\omega}+\frac12\wedgecomm{\boldsymbol\omega}{\boldsymbol\omega})]
\end{align*}

This is a lot similar to Chern-Simons theory,

\begin{align*}
    S_{\textnormal{CS}}\qty[\vb A]&=k\int\limits_M\Tr\qty[\vb A\wedge\dd{\vb A}+\frac13\vb A\wedge\wedgecomm{\vb A}{\vb A}]
\end{align*}

Let's try, $\vb A^x=\boldsymbol\omega+x\vb e$,

\begin{align*}
    S_{\textnormal{CS}}\qty[\vb A^x]&=k\int\limits_M\Tr\qty[\qty(\boldsymbol\omega+x\vb e)\wedge\dd{\qty(\boldsymbol\omega+x\vb e)}+\frac13\qty(\boldsymbol\omega+x\vb e)\wedge\wedgecomm{\boldsymbol\omega+x\vb e}{\boldsymbol\omega+x\vb e}]\\
    S_{\textnormal{CS}}\qty[\vb A^x]&=k\int\limits_M\Tr\biggl[\boldsymbol\omega\wedge\dd{\boldsymbol\omega}+x\boldsymbol\omega\wedge\dd{\vb e}+x\vb e\wedge\dd{\boldsymbol\omega}+x^2\vb e\wedge\dd{\vb e}\\
    &\quad\quad\quad\left.+\frac23\qty(\boldsymbol\omega+x\vb e)\wedge\qty(\boldsymbol\omega+x\vb e)\wedge\qty(\boldsymbol\omega+x\vb e)\right]\\
    S_{\textnormal{CS}}\qty[\vb A^x]&=k\int\limits_M\Tr\biggl[\boldsymbol\omega\wedge\dd{\boldsymbol\omega}+x\dd{\vb e}\wedge\boldsymbol\omega+x\vb e\wedge\dd{\boldsymbol\omega}-\frac12x^2\dd{\qty(\vb e\wedge\vb e)}\\
    &\quad\quad\quad\left.+\frac23\boldsymbol\omega\wedge\boldsymbol\omega\wedge\boldsymbol\omega+2x\boldsymbol\omega\wedge\boldsymbol\omega\wedge\vb e+2x^2\vb e\wedge\vb e\wedge \boldsymbol\omega+\frac23x^3\vb e\wedge\vb e\wedge\vb e\right]\\
    S_{\textnormal{CS}}\qty[\vb A^x]&=k\int\limits_M\Tr\left[\boldsymbol\omega\wedge\qty(\dd{\boldsymbol\omega}+\frac23\boldsymbol\omega\wedge\boldsymbol\omega)+x\dd{\qty(\vb e\wedge\boldsymbol\omega)}+x\vb e\wedge\dd{\boldsymbol\omega}+x\vb e\wedge\qty(\dd{\boldsymbol\omega}+2\boldsymbol\omega\wedge\boldsymbol\omega)+2x^2\vb e\wedge\boldsymbol\omega\wedge\vb e\right.\\
    &\quad\quad\quad\left.+\frac23x^3\vb e\wedge\vb e\wedge\vb e\right]\\
    S_{\textnormal{CS}}\qty[\vb A^x]&=S_{\textnormal{CS}}\qty[\boldsymbol\omega]+k\int\limits_M\Tr\qty[x\dd{\qty(\vb e\wedge\boldsymbol\omega)}+2x\vb e\wedge\qty(\dd{\boldsymbol\omega}+\boldsymbol\omega\wedge\boldsymbol\omega)+2x^2\vb e\wedge\boldsymbol\omega\wedge\vb e+\frac23x^3\vb e\wedge\vb e\wedge\vb e]\\
    S_{\textnormal{CS}}\qty[\vb A^x]&=S_{\textnormal{CS}}\qty[\boldsymbol\omega]+k\int\limits_M\Tr\qty[x\dd{\qty(\vb e\wedge\boldsymbol\omega)}+2x\vb e\wedge\vb R+2x^2\vb e\wedge\boldsymbol\omega\wedge\vb e+\frac23x^3\vb e\wedge\vb e\wedge\vb e]\\
    S_{\textnormal{CS}}\qty[\vb A^x]&=S_{\textnormal{CS}}\qty[\boldsymbol\omega]-4xk\kappa S_{\textnormal{EH}}+k\int\limits_M\Tr\qty[x\dd{\qty(\vb e\wedge\boldsymbol\omega)}+2x^2\vb e\wedge\boldsymbol\omega\wedge\vb e+\frac23x^3\vb e\wedge\vb e\wedge\vb e]
\end{align*}

We can simplify if we sum two contributions,

\begin{align*}
    S_{\textnormal{CS}}\qty[\vb A^x]-S_{\textnormal{CS}}\qty[\vb A^{-x}]&=-8xk\kappa S_{\textnormal{EH}}+2kx\int\limits_{\partial M}\Tr\qty[\vb e\wedge\boldsymbol\omega]+\frac43x^3k\int\limits_M\Tr\qty[\vb e\wedge\vb e\wedge\vb e]\\
    \frac{1}{8xk\kappa}\qty(S_{\textnormal{CS}}\qty[\vb A^{-x}]-S_{\textnormal{CS}}\qty[\vb A^x])&=S_{\textnormal{EH}}-\frac{1}{4\kappa}\int\limits_{\partial M}\Tr\qty[\vb e\wedge\boldsymbol\omega]-\frac{x^2}{3!\kappa}\int\limits_M\Tr\qty[\vb e\wedge\vb e\wedge\vb e]
\end{align*}

And also the not so usual action,

\begin{align*}
    S_{\textnormal{CS}}\qty[\vb A^x]+S_{\textnormal{CS}}\qty[\vb A^{-x}]&=2S_{\textnormal{CS}}\qty[\boldsymbol\omega]+4x^2k\int\limits_M\Tr\qty[\vb e\wedge\boldsymbol\omega\wedge\vb e]
\end{align*}

Chern-Simons Equation of Motion,

\begin{align*}
    S_{\textnormal{CS}}\qty[\vb A+\delta\vb A]-S_{\textnormal{CS}}\qty[\vb A]&=k\int\limits_M\Tr\qty[\delta\vb A\wedge\dd{\vb A}+\vb A\wedge\dd{\delta\vb A}+\frac23\delta\vb A\wedge\vb A\wedge\vb A+\frac23\vb A\wedge\delta\vb A\wedge\vb A+\frac23\vb A\wedge\vb A\wedge\delta\vb A]\\
    S_{\textnormal{CS}}\qty[\vb A+\delta\vb A]-S_{\textnormal{CS}}\qty[\vb A]&=k\int\limits_M\Tr\qty[\dd{\vb A}\wedge\delta\vb A-\dd{\qty(\vb A\wedge\delta\vb A)}+\dd{\vb A}\wedge\delta \vb A+2\vb A\wedge\vb A\wedge\delta\vb A]\\
    S_{\textnormal{CS}}\qty[\vb A+\delta\vb A]-S_{\textnormal{CS}}\qty[\vb A]&=2k\int\limits_M\Tr\qty[\qty(\dd{\vb A}+\vb A\wedge\vb A)\wedge\delta\vb A]-k\int\limits_M\Tr\qty[\dd{\qty(\vb A\wedge\delta\vb A)}]\\
    S_{\textnormal{CS}}\qty[\vb A+\delta\vb A]-S_{\textnormal{CS}}\qty[\vb A]&=2k\int\limits_M\Tr\qty[\vb F\wedge\delta\vb A]-k\int\limits_{\partial M}\Tr\qty[\vb A\wedge\delta\vb A]
\end{align*}

Chern-Simons Gauge Invariance,

\begin{align*}
    S_{\textnormal{CS}}\qty[g\vb Ag^{-1}+g\dd{g^{-1}}]&=k\int\limits_M\Tr\qty[\qty(g\vb Ag^{-1}+g\dd{g^{-1}})\wedge g \vb Fg^{-1}-\frac13\qty(g\vb Ag^{-1}+g\dd{g^{-1}})\wedge\qty(g\vb Ag^{-1}+g\dd{g^{-1}})\wedge\qty(g\vb Ag^{-1}+g\dd{g^{-1}})]\\
    S_{\textnormal{CS}}\qty[g\vb Ag^{-1}+g\dd{g^{-1}}]&=k\int\limits_M\Tr\left[\vb A\wedge\vb F+\dd{g^{-1}}g\wedge \vb F-\frac13\vb A\wedge\vb A\wedge\vb A-\frac13g\dd{g^{-1}}\wedge g\dd{g^{-1}}\wedge g\dd{g^{-1}}\right.\\
    &\quad\quad\quad\left.-g\vb Ag^{-1}\wedge g\vb Ag^{-1}\wedge g\dd{g^{-1}}-g\vb A g^{-1}\wedge g\dd{g^{-1}}\wedge g\dd{g^{-1}}\right]\\
    S_{\textnormal{CS}}\qty[g\vb Ag^{-1}+g\dd{g^{-1}}]&=S_{\textnormal{CS}}\qty[\vb A]+k\int\limits_M\Tr\left[\dd{g^{-1}}g\wedge \vb F-\frac13\dd{g^{-1}}g\wedge \dd{g^{-1}}g\wedge \dd{g^{-1}}g\right.\\
    &\quad\quad\quad\left.-\dd{g^{-1}}g\wedge\vb A\wedge \vb A-\vb A \wedge \dd{g^{-1}}g\wedge \dd{g^{-1}}g\right]\\
    S_{\textnormal{CS}}\qty[g\vb Ag^{-1}+g\dd{g^{-1}}]&=S_{\textnormal{CS}}\qty[\vb A]+k\int\limits_M\Tr\left[\dd{g^{-1}}g\wedge \dd{\vb A}-\frac13\dd{g^{-1}}g\wedge \dd{g^{-1}}g\wedge \dd{g^{-1}}g+\dd{g^{-1}}g\wedge g^{-1}\dd{g}\wedge\vb A \right]\\
    S_{\textnormal{CS}}\qty[g\vb Ag^{-1}+g\dd{g^{-1}}]&=S_{\textnormal{CS}}\qty[\vb A]+k\int\limits_M\Tr\left[\dd{g^{-1}}g\wedge \dd{\vb A}-\frac13\dd{g^{-1}}g\wedge \dd{g^{-1}}g\wedge \dd{g^{-1}}g-\dd{\qty(\dd{g^{-1}}g\wedge\vb A )}-\dd{g^{-1}}g\wedge\dd{\vb A}\right]\\
    S_{\textnormal{CS}}\qty[g\vb Ag^{-1}+g\dd{g^{-1}}]&=S_{\textnormal{CS}}\qty[\vb A]-k\int\limits_M\Tr\left[\frac13\dd{g^{-1}}g\wedge \dd{g^{-1}}g\wedge \dd{g^{-1}}g+\dd{\qty(\dd{g^{-1}}g\wedge\vb A )}\right]
\end{align*}