\section{Introduction}

Einstein-Hilbert action:

\begin{align*}
    S_{\textnormal{EH}}&=\frac{1}{\kappa^2}\int\limits_M\dd[D]{x}\sqrt{\abs{g}}g^{ab}\tensor{R}{_c_b^c_a}
\end{align*}

The Vierbein/Tetrad formalism:

\begin{align*}
    \eta_{\mu\nu}&=\vb g\qty(\vb e_\mu,\vb e_\nu)\\
    g_{ab}&=\tensor{e}{^\mu_a} \tensor{e}{^\nu_b}\eta_{\mu\nu}\\
    \eta_{\mu\nu}&=\tensor{e}{_\mu^a}\tensor{e}{_\nu^b}g_{ab}
\end{align*}

A connection is defined with respect to a vector basis:

\begin{align*}
    \nabla_{\vb X}\qty(\vb e_\nu)&=\tensor{{\boldsymbol\omega(\vb X)}}{^\mu_\nu}\vb e_\mu\\
    \nabla_{\vb X}\qty(\vb e_\nu)&=X^a\tensor{\omega}{_a^\mu_\nu}\vb e_\mu\\
    \vb g\qty(\vb e_\alpha,\nabla_{\vb X}\qty(\vb e_\nu))&=X^a\tensor{\omega}{_a^\mu_\nu}\vb g\qty(\vb e_\alpha,\vb e_\mu)\\
    \vb g\qty(\vb e_\alpha,\nabla_{\vb X}\qty(\vb e_\nu))+\vb g\qty(\vb e_\nu,\nabla_{\vb X}\qty(\vb e_\alpha))&=X^a\tensor{\omega}{_a^\mu_\nu}\vb g\qty(\vb e_\alpha,\vb e_\mu)+X^a\tensor{\omega}{_a^\mu_\alpha}\vb g\qty(\vb e_\nu,\vb e_\mu)\\
    \vb g\qty(\vb e_\alpha,\nabla_{\vb X}\qty(\vb e_\nu))+\vb g\qty(\nabla_{\vb X}\qty(\vb e_\alpha),\vb e_\nu)&=X^a\tensor{\omega}{_a_\alpha_\nu}+X^a\tensor{\omega}{_a_\nu_\alpha}\\
    \tensor{e}{_\alpha^c}g_{cb}\nabla_a\vb e_\nu&=\tensor{e}{_\alpha^c}g_{cb}\tensor{\omega}{_a^\mu_\nu}\vb e_\mu\\
    \tensor{e}{_\alpha^c}g_{cb}\nabla_a\vb e_\nu+\tensor{e}{_\alpha^c}\vb e_\nu\nabla_ag_{cb}&=\tensor{\omega}{_a_\alpha_\nu}\\
    \tensor{e}{_\alpha^c}\nabla_a\qty(g_{cb}\tensor{e}{_\nu^b})&=\tensor{\omega}{_a_\alpha_\nu}\\
    \nabla_a\qty(\tensor{e}{_\alpha^c}g_{cb}\tensor{e}{_\nu^b})-g_{cb}\tensor{e}{_\nu^b}\nabla_a\tensor{e}{_\alpha^c}&=\tensor{\omega}{_a_\alpha_\nu}\\
    \nabla_a\qty(\eta_{\alpha\nu})-g_{cb}\tensor{e}{_\nu^b}\nabla_a\tensor{e}{_\alpha^c}&=\tensor{\omega}{_a_\alpha_\nu}\\
    -g_{cb}\tensor{e}{_\nu^b}\nabla_a\tensor{e}{_\alpha^c}&=\tensor{\omega}{_a_\alpha_\nu}\\
    -\tensor{\omega}{_a_\nu_\alpha}&=\tensor{\omega}{_a_\alpha_\nu},\ \ \ \textnormal{Metric compatibility}\numberthis
\end{align*}

Riemann curvature tensor, $\textbf{Riem}\qty(\vb X,\vb Y):\mathfrak X\rightarrow\mathfrak X$:

\begin{align*}
    \textbf{Riem}\qty(\vb X,\vb Y)\vb e_\mu&=\qty(\nabla_{\vb X}\nabla_{\vb Y}-\nabla_{\vb Y}\nabla_{\vb X}-\nabla_{\comm{\vb X}{\vb Y}})\vb e_\mu\\
    \textbf{Riem}\qty(\vb X,\vb Y)\vb e_\mu&=\qty(\nabla_{\vb X}\qty(Y^b\tensor{\omega}{_b^\nu_\mu}\vb e_\nu)-\nabla_{\vb Y}\qty(X^a\tensor{\omega}{_a^\nu_\mu}\vb e_\nu)-\comm{\vb X}{\vb Y}^b\tensor{\omega}{_b^\nu_\mu}\vb e_\nu)\\
    \textbf{Riem}\qty(\vb X,\vb Y)\vb e_\mu&=\qty(\nabla_{\vb X}\qty(Y^b\tensor{\omega}{_b^\nu_\mu}\vb e_\nu)-\nabla_{\vb Y}\qty(X^a\tensor{\omega}{_a^\nu_\mu}\vb e_\nu)-\comm{\vb X}{\vb Y}^b\tensor{\omega}{_b^\nu_\mu}\vb e_\nu)\\
    \textbf{Riem}\qty(\vb X,\vb Y)\vb e_\mu&=\left(Y^b\nabla_{\vb X}\qty(\tensor{\omega}{_b^\nu_\mu}\vb e_\nu)-X^a\nabla_{\vb Y}\qty(\tensor{\omega}{_a^\nu_\mu}\vb e_\nu)\right.\\
    &\quad\quad\quad\left.+\nabla_{\vb X}\qty(Y^b)\tensor{\omega}{_b^\nu_\mu}\vb e_\nu-\nabla_{\vb Y}\qty(X^b)\tensor{\omega}{_b^\nu_\mu}\vb e_\nu-\comm{\vb X}{\vb Y}^b\tensor{\omega}{_b^\nu_\mu}\vb e_\nu\right)\\
    \textbf{Riem}\qty(\vb X,\vb Y)\vb e_\mu&=\left(X^aY^b\nabla_{a}\qty(\tensor{\omega}{_b^\nu_\mu}\vb e_\nu)-X^aY^b\nabla_{b}\qty(\tensor{\omega}{_a^\nu_\mu}\vb e_\nu)\right.\\
    &\quad\quad\quad\left.+\qty(\nabla_{\vb X}\qty(Y^b)-\nabla_{\vb Y}\qty(X^b))\tensor{\omega}{_b^\nu_\mu}\vb e_\nu-\comm{\vb X}{\vb Y}^b\tensor{\omega}{_b^\nu_\mu}\vb e_\nu\right)\\
    \textbf{Riem}\qty(\vb X,\vb Y)\vb e_\mu&=\left(X^aY^b\nabla_{a}\qty(\tensor{\omega}{_b^\nu_\mu})\vb e_\nu+X^aY^b\tensor{\omega}{_b^\nu_\mu}\tensor{\omega}{_a^\alpha_\nu}\vb e_\alpha-X^aY^b\nabla_{b}\qty(\tensor{\omega}{_a^\nu_\mu})\vb e_\nu-X^aY^b\tensor{\omega}{_a^\nu_\mu}\tensor{\omega}{_b^\alpha_\nu}\vb e_\alpha)\right.\\
    &\quad\quad\quad\left.+\qty(X^a\partial_a Y^b+X^a\tensor{\Gamma}{_a^b_c}Y^c-Y^a\partial_aX^b-Y^a\tensor{\Gamma}{_a^b_c}X^c)\tensor{\omega}{_b^\nu_\mu}\vb e_\nu-\qty(X^a\partial_aY^b-Y^a\partial_a X^b)\tensor{\omega}{_b^\nu_\mu}\vb e_\nu\right)\\
    \textbf{Riem}\qty(\vb X,\vb Y)\vb e_\mu&=X^aY^b\left(\nabla_{a}\qty(\tensor{\omega}{_b^\nu_\mu})+\tensor{\omega}{_b^\alpha_\mu}\tensor{\omega}{_a^\nu_\alpha}-\nabla_{b}\qty(\tensor{\omega}{_a^\nu_\mu})-\tensor{\omega}{_a^\alpha_\mu}\tensor{\omega}{_b^\nu_\alpha}+\tensor{\Gamma}{_a^c_b}\tensor{\omega}{_c^\nu_\mu}-\tensor{\Gamma}{_b^c_a}\tensor{\omega}{_c^\nu_\mu}\right)\vb e_\nu\\
    \textbf{Riem}\qty(\vb X,\vb Y)\vb e_\mu&=X^aY^b\left(\partial_{a}\tensor{\omega}{_b^\nu_\mu}-\partial_{b}\tensor{\omega}{_a^\nu_\mu}+\tensor{\omega}{_a^\nu_\alpha}\tensor{\omega}{_b^\alpha_\mu}-\tensor{\omega}{_b^\nu_\alpha}\tensor{\omega}{_a^\alpha_\mu}\right)\vb e_\nu\\
    \textbf{Riem}\qty(\vb X,\vb Y)\vb e_\mu&=X^aY^b\tensor{\left(\dd{\boldsymbol\omega}+\boldsymbol\omega\wedge\boldsymbol\omega\right)}{_a_b^\nu_\mu}\vb e_\nu\\
    \textbf{Riem}\qty(\vb X,\vb Y)\vb e_\mu&=X^aY^b\tensor{R}{_a_b^\nu_\mu}\vb e_\nu\\
    \textbf{Riem}\qty(\vb X,\vb Y)\qty(\tensor{e}{_\mu^e}\boldsymbol\partial_e)&=X^aY^b\tensor{R}{_a_b^\nu_\mu}\tensor{e}{_\nu^c}\boldsymbol\partial_c\\
    \tensor{e}{_\mu^e}\textbf{Riem}\qty(\vb X,\vb Y)\boldsymbol\partial_e&=X^aY^b\tensor{R}{_a_b^\nu_\mu}\tensor{e}{_\nu^c}\boldsymbol\partial_c\\
    \tensor{e}{_\mu^e}X^aY^b\tensor{R}{_a_b^c_e}\boldsymbol\partial_c&=X^aY^b\tensor{R}{_a_b^\nu_\mu}\tensor{e}{_\nu^c}\boldsymbol\partial_c\\
    \tensor{e}{^\mu_d}\tensor{e}{_\mu^e}\tensor{R}{_a_b^c_e}&=\tensor{e}{^\mu_d}\tensor{R}{_a_b^\nu_\mu}\tensor{e}{_\nu^c}\\
    \tensor{R}{_a_b^c_d}&=\tensor{e}{^\mu_d}\tensor{R}{_a_b^\nu_\mu}\tensor{e}{_\nu^c}
\end{align*}

In the EH action,

\begin{align*}
    S_{\textnormal{EH}}&=\frac{1}{\kappa^2}\int\limits_M\dd[D]{x}\sqrt{\abs{g}}g^{ab}\tensor{R}{_c_b^c_a}\\
    S_{\textnormal{EH}}&=\frac{1}{\kappa^2}\int\limits_M\dd[D]{x}\sqrt{\abs{g}}g^{ab}\tensor{e}{^\mu_a}\tensor{R}{_c_b^\nu_\mu}\tensor{e}{_\nu^c}\\
    S_{\textnormal{EH}}&=\frac{1}{\kappa^2}\int\limits_M\dd[D]{x}\sqrt{\abs{g}}g^{ab}g^{cd}\tensor{e}{^\mu_a}\tensor{R}{_c_b_\nu_\mu}\tensor{e}{^\nu_d}\\
    S_{\textnormal{EH}}&=\frac{1}{2\kappa^2}\int\limits_M\dd[D]{x}\sqrt{\abs{g}}\qty(g^{ab}g^{dc}-g^{ac}g^{db})\tensor{e}{^\mu_a}\tensor{R}{_c_b_\nu_\mu}\tensor{e}{^\nu_d}\\
    S_{\textnormal{EH}}&=\frac{1}{2\qty(D-2)!\kappa^2}\int\limits_M\dd[D]{x}\sqrt{\abs{g}}\epsilon^{a_1\cdots a_{D-2}ad}\tensor{\epsilon}{_{a_1\cdots a_{D-2}}^b^c}\tensor{e}{^\mu_a}\tensor{R}{_c_b_\nu_\mu}\tensor{e}{^\nu_d}\\
    S_{\textnormal{EH}}&=-\frac{1}{2\qty(D-2)!\kappa^2}\int\limits_M\dd[D]{x}\sqrt{\abs{g}}\epsilon^{ada_1\cdots a_{D-2}}\tensor{\epsilon}{^b^c_{a_1\cdots a_{D-2}}}\tensor{e}{^\nu_a}\tensor{R}{_b_c_\nu_\mu}\tensor{e}{^\mu_d}\\
    S_{\textnormal{EH}}&=-\frac{1}{2\kappa^2}\int\limits_M\dd[D]{x}\epsilon^{ada_1\cdots a_{D-2}}\tensor{e}{^\nu_a}\tensor{{\star R}}{_{a_1\cdots a_{D-2}}_\nu_\mu}\tensor{e}{^\mu_d}\\
    S_{\textnormal{EH}}&=-\frac{1}{2\kappa^2}\int\limits_M\frac{1}{D!}\epsilon_{b_1\cdots b_D}\dd{x^{b_1}}\wedge\cdots\wedge\dd{x^{b_D}}\epsilon^{ada_1\cdots a_{D-2}}\tensor{e}{^\nu_a}\tensor{{\star R}}{_{a_1\cdots a_{D-2}}_\nu_\mu}\tensor{e}{^\mu_d}\\
    S_{\textnormal{EH}}&=-\frac{1}{2\kappa^2}\int\limits_M\dd{x^{b_1}}\wedge\cdots\wedge\dd{x^{b_D}}\tensor{g}{_{b_1}^{[a}}\tensor{g}{_{b_2}^{d}}\tensor{g}{_{b_3}^{a_1}}\cdots\tensor{g}{_{b_D}^{a_{D-2}]}}\tensor{e}{^\nu_a}\tensor{{\star R}}{_{a_1\cdots a_{D-2}}_\nu_\mu}\tensor{e}{^\mu_d}\\
    S_{\textnormal{EH}}&=-\frac{1}{2\kappa^2}\int\limits_M\dd{x^{a}}\wedge\dd{x^{d}}\wedge\dd{x^{a_1}}\wedge\cdots\wedge\dd{x^{a_{D-2}}}\tensor{e}{^\nu_a}\tensor{e}{^\mu_d}\tensor{{\star R}}{_{a_1\cdots a_{D-2}}_\nu_\mu}\\
    S_{\textnormal{EH}}&=-\frac{1}{2\kappa^2}\int\limits_M\tensor{e}{^\nu_a}\dd{x^{a}}\wedge\tensor{e}{^\mu_d}\dd{x^{d}}\wedge\dd{x^{a_1}}\wedge\cdots\wedge\dd{x^{a_{D-2}}}\tensor{{\star R}}{_{a_1\cdots a_{D-2}}_\nu_\mu}\\
    S_{\textnormal{EH}}&=-\frac{1}{2\kappa^2}\int\limits_M{\tilde{\vb e}^\nu}\wedge{\tilde{\vb e}^\mu}\wedge\tensor{{\star \textbf{R}}}{_\nu_\mu}
\end{align*}















% Metric:

% \begin{align*}
%     \dd{s}^2&=-A\qty(r)\dd{t}^2+\frac{1}{A\qty(r)}\dd{r}^2+r^2\dd{\Omega}^2\\
%     A\qty(r)&=-B\qty(2-3b_1B)\frac1r+\qty(1-3b_1B)+b_1r+b_2r^2
% \end{align*}

% Ricci:

% \begin{align*}
%     R&=6b_1\qty(B-r)\frac{1}{r^2}-12b_2\\
%     R'&=-12\frac{b_1}{r^3}\qty(B-\frac12r)
% \end{align*}

% Equation:

% \begin{align*}
%     6\beta\square R&=\gamma R+4\gamma\Lambda\\
%     \dv{}{r}\qty(A\qty(r)r^2R')&=\frac{\gamma}{6\beta}\qty( R+4\Lambda)r^2\\
%     -12b_1\dv{}{r}\qty(A\qty(r)\frac1r\qty(B-\frac12 r))&=\frac{\gamma}{6\beta}\qty( 6b_1\qty(B-r)\frac{1}{r^2}-12b_2+4\Lambda)r^2\\
%     -12b_1\dv{}{r}\qty(\qty(-B\qty(2-3b_1B)\frac1r+\qty(1-3b_1B)+b_1r+b_2r^2)\qty(\frac Br-\frac12))&=\frac{\gamma}{6\beta}\qty( 6b_1\qty(B-r)\frac{1}{r^2}-12b_2+4\Lambda)r^2\\
%     -12b_1\qty(B\qty(2-3b_1B)\frac{1}{r^2}+b_1+2b_2r)\qty(\frac Br-\frac12)+12b_1\qty(-B\qty(2-3b_1B)\frac{1}{r}+\qty(1-3b_1B)+b_1r+b_2r^2)\frac{B}{r^2}&=\frac{\gamma}{6\beta}\qty( 6b_1\qty(B-r)\frac{1}{r^2}-12b_2+4\Lambda)r^2\\
%     -r^{-3}24b_1B\qty(2-3b_1B)+r^{-2}12b_1B\qty(3-6b_1B)+6b_1^2-12b_1b_2B+r12b_1b_2&=\frac{\gamma}{6\beta}\qty( 6b_1B-6b_1r-4r^2\qty(3b_2-\Lambda))
% \end{align*}

% Thus:
% \begin{align*}
%     B\qty(2-3b_1B)&=0\\
%     6b_1-12b_2B&=\frac\gamma\beta B\\
%     12b_2&=-\frac\gamma\beta \\
%     3b_2&=\Lambda
% \end{align*}