\section{Conformal Toy Model}

Consider the following Lagrangian, 
\[\mathcal L=-\frac12\Box \phi\Box\phi-\frac{g}{2}\phi^2\Box\phi-\frac{g^2}{8}\phi^4+m^2\qty(-\frac12\partial_\mu\phi\partial^\mu\phi+\frac{g}{3!}\phi^3)\]
Notice the form of the Lagrangian,
\[\mathcal L=-\frac12\qty(\Box\phi+\frac{g}{2}\phi^2)^2+m^2\qty(-\frac12\partial_\mu\phi\partial^\mu\phi+\frac{g}{3!}\phi^3)\]
It possesses the Feynman rules,
\begin{itemize}
    \item \ \ \feynmandiagram [horizontal=a to b] {
		a [particle=\(\phi\)] -- [scalar] b [particle=\(\phi\)],
		}; $=\frac1\im\frac{1}{m^2p^2+p^4}$
	\item \ \ \feynmandiagram [small,baseline = (b.base),horizontal=a to b] {
		a [particle=\(\phi_1\)] -- [scalar] b  ,
		b -- [scalar] c [particle=\(\phi_2\)],
		b -- [scalar] d [particle=\(\phi_3\)],
		}; $=\im g\qty(p_1^2+p_2^2+p_3^2+m^2)$
	\item \ \ \feynmandiagram [small,baseline = (b.base)] {
		a [particle=\(\phi_1\)] -- [scalar] b  ,
		e [particle=\(\phi_1\)] -- [scalar] b  ,
		b -- [scalar] c [particle=\(\phi_2\)],
		b -- [scalar] d [particle=\(\phi_3\)],
		}; $=-3\im g^2$
\end{itemize}

Let's compute the self energy,
\begin{align}
    \im\Pi\qty(p^2)&=\feynmandiagram [baseline = (b.base),horizontal=a to b,layered layout] {
     a -- [scalar] b -- [ loop,scalar,min distance =2cm] b--[scalar] c,
     }; + \feynmandiagram [baseline = (b.base),horizontal=a to b,layered layout] {
     a -- [scalar] b -- [ half left,scalar] c --[half left,scalar] b,
     c -- [scalar] d,
     };+\cdots
\end{align}

\begin{align}
    \im{\Pi^{\qty(1)}}&=-\frac32\im g^2\int\frac{\dd[D]{\ell}}{\qty(2\pi)^D}\frac{1}{\im}\frac{1}{\ell^2}\frac{1}{\ell^2+m^2}\\
    \im{\Pi^{\qty(1)}}&=-\frac32 g^2\int\frac{\dd[D]{\ell}}{\qty(2\pi)^D}\frac{1}{\ell^2}\frac{1}{\ell^2+m^2}\\
    \im{\Pi^{\qty(1)}}&=-\frac32 g^2\frac{\im}{\qty(4\pi)^{\frac D2}\Gamma\qty(\frac D2)}\qty(m^2)^{\frac D2-2}\frac{\Gamma\qty(2-\frac D2)\Gamma\qty(\frac D2-1)}{\Gamma\qty(1)}\\
    \im{\Pi^{\qty(1)}}&=-\frac32\im g^2\frac{\qty(m^2)^{-\epsilon}\Gamma\qty(\epsilon)\Gamma\qty(1-\epsilon)}{\qty(4\pi)^{2-\epsilon}\Gamma\qty(2-\epsilon)}
\end{align}

\begin{align}
    \im{\Pi^{\qty(2)}}&=\frac12\qty(\im g)^2\int\frac{\dd[D]{\ell}}{\qty(2\pi)^D}\frac{1}{\im^2}\frac{1}{\ell^2\qty(\ell+p)^2}\frac{\qty(m^2+\ell^2+p^2+\qty(\ell+p)^2)^2}{\ell^2+m^2}\frac{1}{\qty(\ell+p)^2+m^2}
\end{align}
For the mass renormalization we can take $p=0$,
\begin{align}
    \im{\Pi^{\qty(2)}}&=\frac12g^2\int\frac{\dd[D]{\ell}}{\qty(2\pi)^D}\frac{\qty(m^2+2\ell^2)^2}{\ell^4\qty(\ell^2+m^2)^2}
\end{align}
Let's compute the four point amplitude for this theory,
\begin{align}
    \feynmandiagram [small,baseline = (b.base),horizontal=b to d] {
		a [particle=\(\phi_1\)] -- [scalar] b  ,
		b -- [scalar] c [particle=\(\phi_2\)],
		b -- [scalar,momentum=\(P\)] d,
        d -- [scalar] e [particle=\(\phi_4\)],
        d -- [scalar] f [particle=\(\phi_3\)]
    }; &=\qty(\im g)^2\frac{\qty(p_1^2+p_2^2+\qty(p_1+p_2)^2+m^2)\qty(p_3^2+p_4^2+\qty(p_3+p_4)^2+m^2)}{\im\qty(p_1+p_2)^2\qty(\qty(p_1+p_2)^2+m^2)}
\end{align}
First let's consider all legs massless,
\begin{align}
    \feynmandiagram [small,baseline = (b.base),horizontal=b to d] {
		a [particle=\(\phi_1\)] -- [scalar] b  ,
		b -- [scalar] c [particle=\(\phi_2\)],
		b -- [scalar,momentum=\(P\)] d,
        d -- [scalar] e [particle=\(\phi_4\)],
        d -- [scalar] f [particle=\(\phi_3\)]
    }; &=\im g^2\frac{\qty(-s+m^2)\qty(-s+m^2)}{\qty(-s)\qty(-s+m^2)}=-\im g^2\frac{\qty(-s+m^2)}{s}
\end{align}
So,
\begin{align}
	\vcenter{\hbox{\usebox{\phifourpoint}}} &=-\im g^2\frac{\qty(-s+m^2)}{s}-\im g^2\frac{\qty(-t+m^2)}{t}-\im g^2\frac{\qty(-u+m^2)}{u}-3\im g^2\\
	\vcenter{\hbox{\usebox{\phifourpoint}}} &=-\im g^2\frac{\qty(-s+m^2)}{s}-\im g^2\frac{\qty(-t+m^2)}{t}-\im g^2\frac{\qty(-u+m^2)}{u}-\im g^2\frac{s}{s}-\im g^2\frac{t}{t}-\im g^2\frac{u}{u}\\
	\vcenter{\hbox{\usebox{\phifourpoint}}} &=-\im g^2m^2\qty(\frac1s+\frac1t+\frac1u)=\im g^2 m^2\qty(\frac{1}{\langle12\rangle[12]}+\frac{1}{\langle14\rangle[14]}+\frac{1}{\langle13\rangle[13]})
\end{align}
Para uma perna massiva, $\phi_4$,
\begin{align}
    \feynmandiagram [small,baseline = (b.base),horizontal=b to d] {
		a [particle=\(\phi_1\)] -- [scalar] b  ,
		b -- [scalar] c [particle=\(\phi_2\)],
		b -- [scalar,momentum=\(P\)] d,
        d -- [scalar] e [particle=\(\phi_4\)],
        d -- [scalar] f [particle=\(\phi_3\)]
    }; &=\qty(\im g)^2\frac{\qty(-s+m^2)\qty(-s)}{\im\qty(-s)\qty(-s+m^2)}=\im g^2
\end{align}
So,
\begin{align}
	\vcenter{\hbox{\usebox{\phifourpoint}}} &=\im g^2+\im g^2+\im g^2-3\im g^2=0
\end{align}
Para duas pernas massivas, $\phi_{3,4}$,
\begin{align}
    \feynmandiagram [small,baseline = (b.base),horizontal=b to d] {
		a [particle=\(\phi_1\)] -- [scalar] b  ,
		b -- [scalar] c [particle=\(\phi_2\)],
		b -- [scalar,momentum=\(P\)] d,
        d -- [scalar] e [particle=\(\phi_4\)],
        d -- [scalar] f [particle=\(\phi_3\)]
    }; &=\qty(\im g)^2\frac{\qty(-s+m^2)\qty(-s-m^2)}{\im\qty(-s)\qty(-s+m^2)}=\im g^2\frac{s+m^2}{s}\\
    \feynmandiagram [small,baseline = (b.base),vertical=b to d] {
		a [particle=\(\phi_2\)] -- [scalar] b  ,
		b -- [scalar] c [particle=\(\phi_3\)],
		b -- [scalar,momentum=\(P\)] d,
        d -- [scalar] e [particle=\(\phi_1\)],
        d -- [scalar] f [particle=\(\phi_4\)]
    }; &=\qty(\im g)^2\frac{\qty(-t)\qty(-t)}{\im\qty(-t)\qty(-t+m^2)}=-\im g^2\frac{t}{-t+m^2}\\
    \feynmandiagram [small,baseline = (b.base),vertical=b to d] {
		a [particle=\(\phi_2\)] -- [scalar] b  ,
		b -- [scalar] c [particle=\(\phi_4\)],
		b -- [scalar,momentum=\(P\)] d,
        d -- [scalar] e [particle=\(\phi_1\)],
        d -- [scalar] f [particle=\(\phi_3\)]
    }; &=-\im g^2\frac{u}{-u+m^2}
\end{align}
So,
\begin{align}
	\vcenter{\hbox{\usebox{\phifourpoint}}} &=\im g^2\frac{s+m^2}{s}-\im g^2\frac{t}{-t+m^2}-\im g^2\frac{u}{-u+m^2}-3\im g^2\\
	\vcenter{\hbox{\usebox{\phifourpoint}}} &=\im g^2\frac{s+m^2}{s}-\im g^2\frac{t}{-t+m^2}-\im g^2\frac{u}{-u+m^2}-\im g^2 \frac{s}{s}-\im g^2\frac{-t+m^2}{-t+m^2}-\im g^2\frac{-u+m^2}{-u+m^2}\\
	\vcenter{\hbox{\usebox{\phifourpoint}}} &=-\im g^2 m^2\qty(-\frac{1}{s}+\frac{1}{-t+m^2}+\frac{1}{-u+m^2})=-\im g^2 m^2\qty(\frac{1}{\langle12\rangle[12]}+\frac{1}{\langle1\vb4\rangle[1\vb 4]}+\frac{1}{\langle1\vb3\rangle[1\vb3]})
\end{align}
Para uma perna sem massa $\phi_1$,
\begin{align}
    \feynmandiagram [small,baseline = (b.base),horizontal=b to d] {
		a [particle=\(\phi_1\)] -- [scalar] b  ,
		b -- [scalar] c [particle=\(\phi_2\)],
		b -- [scalar,momentum=\(P\)] d,
        d -- [scalar] e [particle=\(\phi_4\)],
        d -- [scalar] f [particle=\(\phi_3\)]
    }; &=\qty(\im g)^2\frac{\qty(-s)\qty(-s-m^2)}{\im\qty(-s)\qty(-s+m^2)}=-\im g^2\frac{s+m^2}{-s+m^2}\\
    \feynmandiagram [small,baseline = (b.base),vertical=b to d] {
		a [particle=\(\phi_2\)] -- [scalar] b  ,
		b -- [scalar] c [particle=\(\phi_3\)],
		b -- [scalar,momentum=\(P\)] d,
        d -- [scalar] e [particle=\(\phi_1\)],
        d -- [scalar] f [particle=\(\phi_4\)]
    }; &=\qty(\im g)^2\frac{\qty(-t)\qty(-t-m^2)}{\im\qty(-t)\qty(-t+m^2)}=-\im g^2\frac{t+m^2}{-t+m^2}\\
    \feynmandiagram [small,baseline = (b.base),vertical=b to d] {
		a [particle=\(\phi_2\)] -- [scalar] b  ,
		b -- [scalar] c [particle=\(\phi_4\)],
		b -- [scalar,momentum=\(P\)] d,
        d -- [scalar] e [particle=\(\phi_1\)],
        d -- [scalar] f [particle=\(\phi_3\)]
    }; &=\qty(\im g)^2\frac{\qty(-u)\qty(-u-m^2)}{\im\qty(-u)\qty(-u+m^2)}=-\im g^2\frac{u+m^2}{-u+m^2}\\
\end{align}
So,
\begin{align}
	\vcenter{\hbox{\usebox{\phifourpoint}}} &=-\im g^2\frac{s+m^2}{-s+m^2}-\im g^2\frac{t+m^2}{-t+m^2}-\im g^2\frac{u+m^2}{-u+m^2}-3\im g^2\\
	\vcenter{\hbox{\usebox{\phifourpoint}}} &=-\im g^2\frac{s+m^2}{-s+m^2}-\im g^2\frac{t+m^2}{-t+m^2}-\im g^2\frac{u+m^2}{-u+m^2}-\im g^2\frac{-s+m^2}{-s+m^2}-\im g^2\frac{-t+m^2}{-t+m^2}-\im g^2\frac{-u+m^2}{-u+m^2}\\
	\vcenter{\hbox{\usebox{\phifourpoint}}} &=-\im g^2m^2\qty(\frac{1}{-s+m^2}+\frac{1}{-t+m^2}+\frac{1}{-u+m^2})=-\im g^2 m^2\qty(\frac{1}{\langle1\vb 2\rangle[1\vb2]}+\frac{1}{\langle1\vb4\rangle[1\vb 4]}+\frac{1}{\langle1\vb3\rangle[1\vb3]})
\end{align}

Cut comparison, only massless legs

\begin{align}
    \feynmandiagram [baseline = (b.base),horizontal=b to h, layered layout,small] {
        a -- [scalar] b [blob],
        f -- [scalar] b ,
        b -- [ scalar, momentum =\(l+3+4\)] g [blob], 
        g --[scalar,momentum =\(l+4\)] h [blob], 
        h --[scalar, momentum=\(l\)] b,
        g -- [scalar] d,
        h -- [scalar] e,
    };&=\frac{\im g^2m^2\qty(\im g m^2)^2}{\qty(\im m^2)^3}\qty(\frac{1}{\langle12\rangle[12]}-\frac{1}{\langle1l\rangle[1l]}-\frac{1}{\langle2l\rangle[2l]})
\end{align}

to solve for the cuts, $l^2=\qty(l+3+4)^2=\qty(l+4)^2=0$,
\begin{align}
    l^2&=0\Rightarrow l=-|l\rangle [l|\\
    0=\qty(l+4)^2&=\langle l4\rangle[l4]=0\Rightarrow |l]=|4]\\
    0=\qty(l+3+4)^2&=\langle lP_{34}\rangle[lP_{34}]+(3+4)^2=\langle l| 3+4|l]+\langle34\rangle[34]=\langle l| 3+4|4]+\langle34\rangle[34]\\
    \langle43\rangle[34]&=-\langle l3\rangle[34]\Rightarrow |l\rangle = -|4\rangle+z|3\rangle\\
    l&=-\qty(-|4\rangle+z|3\rangle)[4|
\end{align}
The cuts are solved by this. Hence,
\begin{align*}
    &=g^4\qty(\frac{1}{\langle12\rangle[12]}-\frac{1}{\langle1l\rangle[1l]}-\frac{1}{\langle2l\rangle[2l]})\\
    &=g^4\qty(\frac{1}{\langle12\rangle[12]}-\frac{1}{\qty(-\langle14\rangle+z\langle13\rangle)[14]}-\frac{1}{\qty(-\langle24\rangle+z\langle23\rangle)[24]})
\end{align*}
Now for internal massive lines,
\begin{align}
    \feynmandiagram [baseline = (b.base),horizontal=b to h, layered layout,small] {
        a -- [scalar] b [blob],
        f -- [scalar] b ,
        b -- [ scalar, momentum =\(l+3+4\)] g [blob], 
        g --[scalar,momentum =\(l+4\)] h [blob], 
        h --[scalar, momentum=\(l\)] b,
        g -- [scalar] d,
        h -- [scalar] e,
    };&=\frac{-\im g^2m^2\qty(-\im g m^2)^2}{\qty(-\im m^2)^3}\qty(\frac{1}{\langle12\rangle[12]}-\frac{1}{\langle1l\rangle[1l]}-\frac{1}{\langle2l\rangle[2l]})
\end{align}
With the cuts being, $l^2=\qty(l+3+4)^2=\qty(l+4)^2=-m^2$,
\begin{align}
    0=(l+4)^2-l^2&=2l\cdot p_4\\
    0=(l+4+3)^2-l^2&=2l\cdot \qty(4+3)+(4+3)^2=2l\cdot p_3+(4+3)^2
\end{align}
As ansatz, $l=|4\rangle [4|+\alpha|4\rangle [3|+\beta|3\rangle[4|$ satisfy both conditions above. The remaining condition is,
\begin{align}
    l^2&=-m^2\\
    -\alpha\beta[43]\langle43\rangle&=-m^2\Rightarrow \alpha=\frac{m^2}{\beta\langle34\rangle[34]}
\end{align}
Setting now $-\beta=z$,
\begin{align}
    l=|4\rangle [4|-\frac{m^2}{z\langle34\rangle[34]}|4\rangle [3|-z|3\rangle[4|
\end{align}
The value of the diagram is,
\begin{align*}
    &=g^4\qty(\frac{1}{\langle12\rangle[12]}+\frac{1}{\langle1l\rangle[l1]}+\frac{1}{\langle2l\rangle[l2]})\\
    &=g^4\qty(\frac{1}{\langle12\rangle[12]}+\frac{1}{-\langle1|l|1]}+\frac{1}{-\langle2|l|2]})\\
    &=g^4\qty(\frac{1}{\langle12\rangle[12]}-\frac{1}{\langle14\rangle[41]-\frac{m^2}{z\langle34\rangle[34]}\langle14\rangle[31]-z\langle13\rangle[41]}-\frac{1}{\langle2|l|2]})
\end{align*}
The explicit cut loop amplitude is,
\begin{align*}
    \feynmandiagram [baseline = (b.base),horizontal=b to g,small] {
        a -- [scalar] b ,
        f -- [scalar] c ,
        b -- [ scalar, momentum =\(l+3+4\)] g , 
        g --[scalar,momentum =\(l+4\)] h , 
        h --[scalar, momentum=\(l\)] c,
        c --[scalar, momentum=\(l-1\)] b,
        g -- [scalar] e,
        h -- [scalar] d,
    };
\end{align*}
Triple cut has no improvement, what about a double cut,

\begin{align}
    \vcenter{\hbox{\usebox{\phifourloop}}}&=\frac{\qty(\im g^2m^2)^2}{\qty(\im m^2)^2}\qty(\frac{1}{\langle12\rangle[12]}-\frac{1}{\langle1\ell\rangle[1\ell]}-\frac{1}{\langle2\ell\rangle[2\ell]})\qty(\frac{1}{\langle34\rangle[34]}+\frac{1}{\langle3\ell\rangle[3\ell]}+\frac{1}{\langle4\ell\rangle[4\ell]})
\end{align}

Five point amplitude,

\begin{align*}
    \feynmandiagram [small] {
        i1 [particle = \(3\)]-- [scalar] v1,
        i2 [particle=\(4\)]-- [scalar] v1,
        v1 -- [scalar] v2,
        v2 -- [scalar] i5 [particle=\(5\)],
        v2 -- [scalar] v3,
        v3 -- [scalar] i3 [particle=\(1\)],
        v3 -- [scalar] i4 [particle=\(2\)]
    }; &=  \frac{\qty(\im g)^3\qty(m^2+p_1^2+p_2^2+\qty(p_1+p_2)^2)\qty(m^2+p_5^2+\qty(p_3+p_4)^2+\qty(p_1+p_2)^2)\qty(m^2+p_3^2+p_4^2+\qty(p_3+p_4)^2)}{i^2\qty(p_1+p_2)^2\qty(\qty(p_1+p_2)^2+m^2)\qty(p_3+p_4)^2\qty(\qty(p_3+p_4)^2+m^2)}
\end{align*}

Let's consider the special case of all massless,

\begin{align*}
    \feynmandiagram [small] {
        i1 [particle = \(3\)]-- [scalar] v1,
        i2 [particle=\(4\)]-- [scalar] v1,
        v1 -- [scalar] v2,
        v2 -- [scalar] i5 [particle=\(5\)],
        v2 -- [scalar] v3,
        v3 -- [scalar] i3 [particle=\(1\)],
        v3 -- [scalar] i4 [particle=\(2\)]
    }; &=\frac{ \im g^3}{\qty(p_1+p_2)^2} \frac{\qty(m^2+\qty(p_3+p_4)^2+\qty(p_1+p_2)^2)\qty(m^2+\qty(p_3+p_4)^2)}{\qty(p_3+p_4)^2\qty(\qty(p_3+p_4)^2+m^2)}=\frac{ \im g^3}{\qty(p_1+p_2)^2} \frac{\qty(m^2+\qty(p_3+p_4)^2+\qty(p_1+p_2)^2)}{\qty(p_3+p_4)^2}
\end{align*}

Combining this graph with,

\begin{align*}
    \feynmandiagram [small] {
        i1 [particle = \(4\)]-- [scalar] v1,
        i2 [particle=\(5\)]-- [scalar] v1,
        v1 -- [scalar] i5 [particle=\(3\)],
        v1 -- [scalar] v2,
        v2 -- [scalar] i3 [particle=\(2\)],
        v2 -- [scalar] i4 [particle=\(1\)]
    }; &=\frac{-\im 3g^2\im g\qty(m^2+\qty(p_1+p_2)^2)}{\im\qty(p_1+p_2)^2\qty(\qty(p_1+p_2)^2+m^2)}=\frac{-3\im g^3}{\qty(p_1+p_2)^2}
\end{align*}

We get,

\begin{align*}
    \feynmandiagram [small] {
        i1 [particle = \(4\)]-- [scalar] v1 [blob],
        i2 [particle=\(5\)]-- [scalar] v1,
        v1 -- [scalar] i5 [particle=\(3\)],
        v1 -- [scalar] v2,
        v2 -- [scalar] i3 [particle=\(2\)],
        v2 -- [scalar] i4 [particle=\(1\)]
    }; &=\frac{ \im g^3}{\qty(p_1+p_2)^2}\qty[ \frac{\qty(m^2+\qty(p_3+p_4)^2+\qty(p_1+p_2)^2)}{\qty(p_3+p_4)^2}-\frac{\qty(p_3+p_4)^2}{\qty(p_3+p_4)^2}+\frac{\qty(m^2+\qty(p_3+p_5)^2+\qty(p_1+p_2)^2)}{\qty(p_3+p_5)^2}-\frac{\qty(p_3+p_5)^2}{\qty(p_3+p_5)^2}+\frac{\qty(m^2+\qty(p_5+p_4)^2+\qty(p_1+p_2)^2)}{\qty(p_5+p_4)^2}-\frac{\qty(p_5+p_4)^2}{\qty(p_5+p_4)^2}]\\
        &=\frac{ \im g^3\qty(m^2+\qty(p_1+p_2)^2)}{\qty(p_1+p_2)^2}\qty[ \frac{1}{\qty(p_3+p_4)^2}+\frac{1}{\qty(p_3+p_5)^2}+\frac{1}{\qty(p_5+p_4)^2}]
\end{align*}

Now we have to sum the contributions of $1$ being in the middle,

\begin{align*}
    \feynmandiagram [small] {
        i1 [particle = \(3\)]-- [scalar] v1,
        i2 [particle=\(4\)]-- [scalar] v1,
        v1 -- [scalar] v2,
        v2 -- [scalar] i5 [particle=\(1\)],
        v2 -- [scalar] v3,
        v3 -- [scalar] i3 [particle=\(5\)],
        v3 -- [scalar] i4 [particle=\(2\)]
    }; + \feynmandiagram [small] {
        i1 [particle = \(4\)]-- [scalar] v1,
        i2 [particle=\(1\)]-- [scalar] v1,
        v1 -- [scalar] i5 [particle=\(3\)],
        v1 -- [scalar] v2,
        v2 -- [scalar] i3 [particle=\(2\)],
        v2 -- [scalar] i4 [particle=\(5\)]
    };+\textnormal{ perm}
\end{align*}

Which will be,

\begin{align*}
    \frac{\im g^3}{\qty(p_2+p_3)^2}\frac{m^2+\qty(p_2+p_3)^2+\qty(p_4+p_5)^2}{\qty(p_4+p_5)^2}-\frac{3\im g^3}{\qty(p_2+p_3)^2}-\frac{3\im g^3}{\qty(p_4+p_5)^2}+\qty(3\leftrightarrow4,5)
\end{align*}

Summing all the contributions we have,

\begin{align*}
    =&\frac{ \im g^3m^2}{\qty(p_1+p_2)^2}\qty[ \frac{1}{\qty(p_3+p_4)^2}+\frac{1}{\qty(p_3+p_5)^2}+\frac{1}{\qty(p_5+p_4)^2}]+\qty(2\leftrightarrow3,4,5)\\
    &\quad\quad\quad+ \im g^3\qty[ \frac{1}{\qty(p_3+p_4)^2}+\frac{1}{\qty(p_3+p_5)^2}+\frac{1}{\qty(p_5+p_4)^2}+\frac{1}{\qty(p_2+p_4)^2}+\frac{1}{\qty(p_2+p_5)^2}+\frac{1}{\qty(p_5+p_4)^2}+\frac{1}{\qty(p_3+p_2)^2}+\frac{1}{\qty(p_3+p_5)^2}+\frac{1}{\qty(p_5+p_2)^2}+\frac{1}{\qty(p_3+p_4)^2}+\frac{1}{\qty(p_3+p_2)^2}+\frac{1}{\qty(p_2+p_4)^2}]\\
    &\quad\quad\quad+ \frac{\im g^3m^2}{\qty(p_2+p_3)^2\qty(p_4+p_5)^2}-\frac{2\im g^3}{\qty(p_2+p_3)^2}-\frac{2\im g^3}{\qty(p_4+p_5)^2}+\qty(3\leftrightarrow4,5)\\
    =&\frac{ \im g^3m^2}{\qty(p_1+p_2)^2}\qty[ \frac{1}{\qty(p_3+p_4)^2}+\frac{1}{\qty(p_3+p_5)^2}+\frac{1}{\qty(p_5+p_4)^2}]+\qty(2\leftrightarrow3,4,5)\\
    &\quad\quad\quad+ \frac{\im g^3m^2}{\qty(p_2+p_3)^2\qty(p_4+p_5)^2}+ \frac{\im g^3m^2}{\qty(p_2+p_4)^2\qty(p_3+p_5)^2}+ \frac{\im g^3m^2}{\qty(p_2+p_5)^2\qty(p_4+p_3)^2}
\end{align*}

By residue, any amplitude with just one massive external on-shell leg is zero. For two massive external on-shell legs, let's take as massive $1,2$,

\begin{align*}
    \feynmandiagram [small] {
        i1 [particle = \(3\)]-- [scalar] v1,
        i2 [particle=\(4\)]-- [scalar] v1,
        v1 -- [scalar] v2,
        v2 -- [scalar] i5 [particle=\(5\)],
        v2 -- [scalar] v3,
        v3 -- [scalar] i3 [particle=\(1\)],
        v3 -- [scalar] i4 [particle=\(2\)]
    }; 
    &= \im g^3\frac{\qty(\qty(p_1+p_2)^2-m^2)}{\qty(p_1+p_2)^2\qty(m^2+\qty(p_1+p_2)^2)}\frac{\qty(m^2+\qty(p_1+p_2)^2+\qty(p_3+p_4)^2)}{\qty(p_3+p_4)^2}
\end{align*}

Combining this graph with,

\begin{align*}
    \feynmandiagram [small] {
        i1 [particle = \(4\)]-- [scalar] v1,
        i2 [particle=\(5\)]-- [scalar] v1,
        v1 -- [scalar] i5 [particle=\(3\)],
        v1 -- [scalar] v2,
        v2 -- [scalar] i3 [particle=\(2\)],
        v2 -- [scalar] i4 [particle=\(1\)]
    }; 
    &=-3\im g^3\frac{\qty(p_1+p_2)^2-m^2}{\qty(p_1+p_2)^2\qty(m^2+\qty(p_1+p_2)^2)}
\end{align*}

so,

\begin{align*}
    \feynmandiagram [small] {
        i1 [particle = \(4\)]-- [scalar] v1 [blob],
        i2 [particle=\(5\)]-- [scalar] v1,
        v1 -- [scalar] i5 [particle=\(3\)],
        v1 -- [scalar] v2,
        v2 -- [scalar] i3 [particle=\(2\)],
        v2 -- [scalar] i4 [particle=\(1\)]
    };
    &=\im g^3\frac{\qty(\qty(p_1+p_2)^2-m^2)}{\qty(p_1+p_2)^2\qty(m^2+\qty(p_1+p_2)^2)}\qty[\frac{\qty(m^2+\qty(p_1+p_2)^2+\qty(p_3+p_4)^2)}{\qty(p_3+p_4)^2}-\frac{\qty(p_3+p_4)^2}{\qty(p_3+p_4)^2}+\qty(5\leftrightarrow3,4)]\\
    &=\im g^3\frac{\qty(\qty(p_1+p_2)^2-m^2)}{\qty(p_1+p_2)^2}\qty[\frac{1}{\qty(p_3+p_4)^2}+\frac{1}{\qty(p_5+p_4)^2}+\frac{1}{\qty(p_3+p_5)^2}]
\end{align*}

The other contributions are,

\begin{align*}
    \feynmandiagram [small] {
        i1 [particle = \(4\)]-- [scalar] v1 [blob],
        i2 [particle=\(5\)]-- [scalar] v1,
        v1 -- [scalar] i5 [particle=\(2\)],
        v1 -- [scalar] v2,
        v2 -- [scalar] i3 [particle=\(3\)],
        v2 -- [scalar] i4 [particle=\(1\)]
    };
    &=\frac{\im g^3\qty(p_1+p_3)^2}{\qty(m^2+\qty(p_1+p_3)^2)}\qty[\frac{1}{m^2+\qty(p_2+p_4)^2}+\frac{1}{m^2+\qty(p_2+p_5)^2}+\frac{1}{(p_4+p_5)^2}]
\end{align*}

Now we have to sum the contributions of $1$ being in the middle,

\begin{align*}
    \feynmandiagram [small] {
        i1 [particle = \(3\)]-- [scalar] v1,
        i2 [particle=\(4\)]-- [scalar] v1,
        v1 -- [scalar] v2,
        v2 -- [scalar] i5 [particle=\(1\)],
        v2 -- [scalar] v3,
        v3 -- [scalar] i3 [particle=\(5\)],
        v3 -- [scalar] i4 [particle=\(2\)]
    }; + \feynmandiagram [small] {
        i1 [particle = \(4\)]-- [scalar] v1,
        i2 [particle=\(1\)]-- [scalar] v1,
        v1 -- [scalar] i5 [particle=\(3\)],
        v1 -- [scalar] v2,
        v2 -- [scalar] i3 [particle=\(2\)],
        v2 -- [scalar] i4 [particle=\(5\)]
    };+\textnormal{ perm}
\end{align*}

which are,

\begin{align*}
    &=\im g^3\frac{\qty(p_2+p_3)^2+\qty(p_4+p_5)^2}{\qty(m^2+\qty(p_2+p_3)^2)\qty(p_4+p_5)^2}-\frac{3\im g^3}{m^2+\qty(p_2+p_3)^2}-\frac{3\im g^3}{\qty(p_4+p_5)^2}+\qty(3\leftrightarrow4,5)
\end{align*}

So, summing all the contributions,

\begin{align*}
    &=\im g^3\frac{\qty(\qty(p_1+p_2)^2-m^2)}{\qty(p_1+p_2)^2}\qty[\frac{1}{\qty(p_3+p_4)^2}+\frac{1}{\qty(p_5+p_4)^2}+\frac{1}{\qty(p_3+p_5)^2}]\\
    &\quad\quad\quad+\frac{\im g^3\qty(p_1+p_3)^2}{\qty(m^2+\qty(p_1+p_3)^2)}\qty[\frac{1}{m^2+\qty(p_2+p_4)^2}+\frac{1}{m^2+\qty(p_2+p_5)^2}+\frac{1}{(p_4+p_5)^2}]+\qty(3\leftrightarrow4,5)\\
    &\quad\quad\quad+\im g^3\frac{\qty(p_2+p_3)^2+\qty(p_4+p_5)^2}{\qty(m^2+\qty(p_2+p_3)^2)\qty(p_4+p_5)^2}-\frac{3\im g^3}{m^2+\qty(p_2+p_3)^2}-\frac{3\im g^3}{\qty(p_4+p_5)^2}+\qty(3\leftrightarrow4,5)\\
    &=-\im g^3\frac{m^2}{\qty(p_1+p_2)^2}\qty[\frac{1}{\qty(p_3+p_4)^2}+\frac{1}{\qty(p_5+p_4)^2}+\frac{1}{\qty(p_3+p_5)^2}]\\
    &\quad\quad\quad+\im g^3\qty[\frac{1}{\qty(p_3+p_4)^2}+\frac{1}{\qty(p_5+p_4)^2}+\frac{1}{\qty(p_3+p_5)^2}]\\
    &\quad\quad\quad+\im g^3\qty[\frac{1}{2p_2\cdot p_4}+\frac{1}{2p_2\cdot p_5}+\frac{1}{(p_4+p_5)^2}]+\qty(3\leftrightarrow4,5)\\
    &\quad\quad\quad-\im g^3\frac{m^2}{\qty(2p_1\cdot p_3)}\qty[\frac{1}{2p_2\cdot p_4}+\frac{1}{2p_2\cdot p_5}+\frac{1}{(p_4+p_5)^2}]+\qty(3\leftrightarrow4,5)\\
    &\quad\quad\quad+\im g^3\frac{-m^2+2p_2\cdot p_3+\qty(p_4+p_5)^2}{\qty(2p_2\cdot p_3)\qty(p_4+p_5)^2}-\frac{3\im g^3}{2p_2\cdot p_3}-\frac{3\im g^3}{\qty(p_4+p_5)^2}+\qty(3\leftrightarrow4,5)\\
    &=-\frac{\im g^3m^2}{\qty(p_1+p_2)^2}\qty[\frac{1}{\qty(p_3+p_4)^2}+\frac{1}{\qty(p_5+p_4)^2}+\frac{1}{\qty(p_3+p_5)^2}]\\
    &\quad\quad\quad+\im g^3\qty[\frac{1}{\qty(p_3+p_4)^2}+\frac{1}{\qty(p_5+p_4)^2}+\frac{1}{\qty(p_3+p_5)^2}]\\
    &\quad\quad\quad+\im g^3\qty[\frac{1}{2p_2\cdot p_4}+\frac{1}{2p_2\cdot p_5}+\frac{1}{(p_4+p_5)^2}+\frac{1}{2p_2\cdot p_3}+\frac{1}{2p_2\cdot p_5}+\frac{1}{(p_3+p_5)^2}+\frac{1}{2p_2\cdot p_4}+\frac{1}{2p_2\cdot p_3}+\frac{1}{(p_4+p_3)^2}]\\
    &\quad\quad\quad-\frac{\im g^3m^2}{\qty(2p_1\cdot p_3)}\qty[\frac{1}{2p_2\cdot p_4}+\frac{1}{2p_2\cdot p_5}+\frac{1}{(p_4+p_5)^2}]+\qty(3\leftrightarrow4,5)\\
    &\quad\quad\quad-\frac{\im g^3m^2}{\qty(2p_2\cdot p_3)\qty(p_4+p_5)^2}+\qty(3\leftrightarrow4,5)\\
    &\quad\quad\quad-\frac{2\im g^3}{2p_2\cdot p_3}-\frac{2\im g^3}{\qty(p_4+p_5)^2}-\frac{2\im g^3}{2p_2\cdot p_4}-\frac{2\im g^3}{\qty(p_3+p_5)^2}-\frac{2\im g^3}{2p_2\cdot p_5}-\frac{2\im g^3}{\qty(p_4+p_3)^2}\\
    &=-\frac{\im g^3m^2}{\qty(p_1+p_2)^2}\qty[\frac{1}{\qty(p_3+p_4)^2}+\frac{1}{\qty(p_5+p_4)^2}+\frac{1}{\qty(p_3+p_5)^2}]\\
    &\quad\quad\quad-\frac{\im g^3m^2}{\qty(2p_1\cdot p_3)}\qty[\frac{1}{2p_2\cdot p_4}+\frac{1}{2p_2\cdot p_5}+\frac{1}{(p_4+p_5)^2}]+\qty(3\leftrightarrow4,5)\\
    &\quad\quad\quad-\frac{\im g^3m^2}{\qty(2p_2\cdot p_3)\qty(p_4+p_5)^2}+\qty(3\leftrightarrow4,5)
\end{align*}

Is almost the same of the all massless, but with a different denominator in the $1,2$ channel. Now with three massive legs, being $3,4,5$,

\begin{align*}
    \feynmandiagram [small] {
        i1 [particle = \(3\)]-- [scalar] v1,
        i2 [particle=\(4\)]-- [scalar] v1,
        v1 -- [scalar] v2,
        v2 -- [scalar] i5 [particle=\(5\)],
        v2 -- [scalar] v3,
        v3 -- [scalar] i3 [particle=\(1\)],
        v3 -- [scalar] i4 [particle=\(2\)]
    }; 
    &= \im g^3\frac{\qty(\qty(p_1+p_2)^2+\qty(p_3+p_4)^2)\qty(-m^2+\qty(p_3+p_4)^2)}{\qty(p_1+p_2)^2\qty(p_3+p_4)^2\qty(m^2+\qty(p_3+p_4)^2)}
\end{align*}

With,

\begin{align*}
    \feynmandiagram [small] {
        i1 [particle = \(4\)]-- [scalar] v1,
        i2 [particle=\(5\)]-- [scalar] v1,
        v1 -- [scalar] i5 [particle=\(3\)],
        v1 -- [scalar] v2,
        v2 -- [scalar] i3 [particle=\(2\)],
        v2 -- [scalar] i4 [particle=\(1\)]
    }; &=\frac{-\im 3g^2\im g\qty(m^2+\qty(p_1+p_2)^2)}{\im\qty(p_1+p_2)^2\qty(\qty(p_1+p_2)^2+m^2)}=\frac{-3\im g^3}{\qty(p_1+p_2)^2}
\end{align*}

So,

\begin{align*}
    \feynmandiagram [small] {
        i1 [particle = \(4\)]-- [scalar] v1 [blob],
        i2 [particle=\(5\)]-- [scalar] v1,
        v1 -- [scalar] i5 [particle=\(3\)],
        v1 -- [scalar] v2,
        v2 -- [scalar] i3 [particle=\(2\)],
        v2 -- [scalar] i4 [particle=\(1\)]
    };
    &=\im g^3\frac{\qty(\qty(p_1+p_2)^2+\qty(p_3+p_4)^2)\qty(-m^2+\qty(p_3+p_4)^2)}{\qty(p_1+p_2)^2\qty(p_3+p_4)^2\qty(m^2+\qty(p_3+p_4)^2)}-\frac{3\im g^3}{\qty(p_1+p_2)^2}\\
    &=\frac{\im g^3}{\qty(p_1+p_2)^2}\qty[\frac{\qty(\qty(p_1+p_2)^2+\qty(p_3+p_4)^2)\qty(-m^2+\qty(p_3+p_4)^2)}{\qty(p_3+p_4)^2\qty(m^2+\qty(p_3+p_4)^2)}-\frac{\qty(p_3+p_4)^2\qty(m^2+\qty(p_3+p_4)^2)}{\qty(p_3+p_4)^2\qty(m^2+\qty(p_3+p_4)^2)}]+\qty(5\leftrightarrow3,4)\\
    &=\frac{\im g^3}{\qty(p_1+p_2)^2}\qty[\frac{\qty(p_1+p_2)^2\qty(-m^2+\qty(p_3+p_4)^2)-2m^2\qty(p_3+p_4)^2}{\qty(p_3+p_4)^2\qty(m^2+\qty(p_3+p_4)^2)}]+\qty(5\leftrightarrow3,4)
\end{align*}