\section{Gamma Matrix Technology}

We start with the trace properties, we're going to assume here that the space-time is `$D$' 
dimensional, except when there is a `$\gamma_5$'. There is a small catch where, as what 
is the dimension of the matrices for an arbitrary space-time dimensionality, the answer is 
`$2^{\lfloor \frac D2\rfloor}$', but as we're always interested in the dimensional regularization, 
this only amounts for an additional finite term in the counter terms, so, we're just assuming 
the matrices are `$4$' dimensional,

\begin{itemize}
    \item $\Tr\qty[\gamma^\mu \gamma^\nu]=4g^{\mu\nu}$
\end{itemize}

This is simple,

\begin{align}
    \acomm{\gamma^\mu}{\gamma^\nu}&=2g^{\mu\nu}\mathbbm 1\nonumber\\
    \Tr\qty[\acomm{\gamma^\mu}{\gamma^\nu}]&=2g^{\mu\nu}\Tr\qty[\mathbbm 1]\nonumber\\
    2\Tr\qty[\gamma^\mu\gamma^\nu]&=8g^{\mu\nu}\nonumber\\
    \Tr\qty[\gamma^\mu\gamma^\nu]&=4g^{\mu\nu}\nonumber
\end{align}

\begin{itemize}
    \item $\Tr\qty[\gamma^\mu \gamma^\nu\gamma^{\alpha}\gamma^{\beta}]=4g^{\mu\beta}g^{\nu\alpha}-4g^{\nu\beta}g^{\alpha\mu}+4g^{\mu\nu}g^{\alpha\beta}$
\end{itemize}

\begin{align}
    \Tr\qty[\gamma^\mu \gamma^\nu\gamma^{\alpha}\gamma^{\beta}]&=\Tr\qty[\gamma^\mu \gamma^\nu\qty(-\gamma^{\beta}\gamma^{\alpha}+2g^{\alpha\beta})]\nonumber\\
    &=-\Tr\qty[\gamma^\mu \gamma^\nu\gamma^{\beta}\gamma^{\alpha}]+8g^{\mu\nu}g^{\alpha\beta}\nonumber\\
    &=-\Tr\qty[\gamma^\mu\qty(- \gamma^\beta\gamma^{\nu}+2g^{\nu\beta})\gamma^{\alpha}]+8g^{\mu\nu}g^{\alpha\beta}\nonumber\\
    &=\Tr\qty[\gamma^\mu\gamma^\beta\gamma^{\nu}\gamma^{\alpha}]-8g^{\nu\beta}g^{\alpha\mu}+8g^{\mu\nu}g^{\alpha\beta}\nonumber\\
    &=\Tr\qty[\qty(-\gamma^\beta\gamma^\mu+2g^{\mu\beta})\gamma^{\nu}\gamma^{\alpha}]-8g^{\nu\beta}g^{\alpha\mu}+8g^{\mu\nu}g^{\alpha\beta}\nonumber\\
    &=-\Tr\qty[\gamma^\beta\gamma^\mu\gamma^{\nu}\gamma^{\alpha}]+8g^{\mu\beta}g^{\nu\alpha}-8g^{\nu\beta}g^{\alpha\mu}+8g^{\mu\nu}g^{\alpha\beta}\nonumber\\
    2\Tr\qty[\gamma^\mu\gamma^{\nu}\gamma^{\alpha}\gamma^\beta]&=8g^{\mu\beta}g^{\nu\alpha}-8g^{\nu\beta}g^{\alpha\mu}+8g^{\mu\nu}g^{\alpha\beta}\nonumber\\
    \Tr\qty[\gamma^\mu\gamma^{\nu}\gamma^{\alpha}\gamma^\beta]&=4g^{\mu\beta}g^{\nu\alpha}-4g^{\nu\beta}g^{\alpha\mu}+4g^{\mu\nu}g^{\alpha\beta}\nonumber
\end{align}

\begin{itemize}
    \item $\Tr\qty[\gamma_5]=0$
\end{itemize}

\begin{align}
    \Tr\qty[\gamma_5]&=\im\Tr\qty[\gamma^0\gamma^1\gamma^2\gamma^3]\nonumber\\
    &=\im4\qty(g^{03}g^{12}-g^{13}g^{20}+g^{01}g^{23})=0\nonumber
\end{align}

Now we'll need another result,

\begin{itemize}
    \item $\acomm{\gamma_5}{\gamma^\mu}=0$
\end{itemize}

This has to be proved case by case,

\begin{align}
    \acomm{\gamma_5}{\gamma^0}&=\im\gamma^0\gamma^1\gamma^2\gamma^3\gamma^0+\im\gamma^0\gamma^0\gamma^1\gamma^2\gamma^3\nonumber\\
    &=-\im\gamma^0\gamma^1\gamma^2\gamma^0\gamma^3-\gamma^1\gamma^2\gamma^3\nonumber\\
    &=\im\gamma^0\gamma^1\gamma^0\gamma^2\gamma^3-\gamma^1\gamma^2\gamma^3\nonumber\\
    &=-\im\gamma^0\gamma^0\gamma^1\gamma^2\gamma^3-\gamma^1\gamma^2\gamma^3\nonumber\\
    &=\im\gamma^1\gamma^2\gamma^3-\gamma^1\gamma^2\gamma^3\nonumber\\
    &=0\nonumber
\end{align}

The proof for the other matrix are analogous,

\begin{itemize}
    \item $\gamma_5\gamma_5=\mathbbm 1$
\end{itemize}

\begin{align}
    \gamma_5\gamma_5&=\im\gamma^0\gamma^1\gamma^2\gamma^3\im\gamma^0\gamma^1\gamma^2\gamma^3\nonumber\\
    &=-\gamma^0\gamma^1\gamma^2\gamma^3\gamma^0\gamma^1\gamma^2\gamma^3\nonumber\\
    &=\gamma^0\gamma^1\gamma^2\gamma^0\gamma^1\gamma^2\gamma^3\gamma^3\nonumber\\
    &=\gamma^0\gamma^1\gamma^0\gamma^1\gamma^2\gamma^2\nonumber\\
    &=-\gamma^0\gamma^0\gamma^1\gamma^1=\mathbbm 1\nonumber
\end{align}

\begin{itemize}
    \item $\Tr\qty[\textnormal{odd number of }\gamma]=0$
\end{itemize}

\begin{align}
    \Tr\qty[\gamma^{\mu_1}\cdots\gamma^{\mu_{2n+1}}]&=\Tr\qty[\gamma^{\mu_1}\cdots\gamma^{\mu_{2n+1}}\gamma_5\gamma_5]\nonumber\\
    &=\qty(-1)^{2n+1}\Tr\qty[\gamma_5\gamma^{\mu_1}\cdots\gamma^{\mu_{2n+1}}\gamma_5]\nonumber\\
    &=-\Tr\qty[\gamma^{\mu_1}\cdots\gamma^{\mu_{2n+1}}]\nonumber\\
    \Tr\qty[\gamma^{\mu_1}\cdots\gamma^{\mu_{2n+1}}]&=0\nonumber
\end{align}

\begin{itemize}
    \item $\Tr\qty[\gamma_5\textnormal{ odd number of }\gamma]=0$
\end{itemize}

\begin{align}
    \Tr\qty[\gamma_5\gamma^{\mu_1}\cdots\gamma^{\mu_{2n+1}}]&=\Tr\qty[\gamma_5\gamma^{\mu_1}\cdots\gamma^{\mu_{2n+1}}\gamma_5\gamma_5]\nonumber\\
    &=\qty(-1)^{2n+1}\Tr\qty[\gamma_5\gamma_5\gamma^{\mu_1}\cdots\gamma^{\mu_{2n+1}}\gamma_5]\nonumber\\
    &=-\Tr\qty[\gamma_5\gamma^{\mu_1}\cdots\gamma^{\mu_{2n+1}}]\nonumber\\
    \Tr\qty[\gamma_5\gamma^{\mu_1}\cdots\gamma^{\mu_{2n+1}}]&=0\nonumber
\end{align}

\begin{itemize}
    \item $\Tr\qty[\gamma_5\gamma^\mu\gamma^\nu]=0$
\end{itemize}

Take `$\alpha\neq \mu$' and `$\alpha\neq \nu$', and the following is not assuming the summation 
convention,

\begin{align}
    \Tr\qty[\gamma_5\gamma^\mu\gamma^\nu]&=\Tr\qty[\gamma_5g_{\alpha\alpha}\gamma^\alpha\gamma^\alpha\gamma^\mu\gamma^\nu]\nonumber\\
    &=-\Tr\qty[\gamma_5g_{\alpha\alpha}\gamma^\alpha\gamma^\mu\gamma^\alpha\gamma^\nu]\nonumber\\
    &=\Tr\qty[\gamma_5g_{\alpha\alpha}\gamma^\alpha\gamma^\mu\gamma^\nu\gamma^\alpha]\nonumber\\
    &=-\Tr\qty[\gamma_5\gamma^\alpha g_{\alpha\alpha}\gamma^\alpha\gamma^\mu\gamma^\nu]\nonumber\\
    \Tr\qty[\gamma_5\gamma^\mu\gamma^\nu]&=0\nonumber
\end{align}

\begin{itemize}
    \item $\Tr\qty[\gamma_5\gamma^\mu\gamma^\nu\gamma^\alpha\gamma^\beta]=4\im\epsilon^{\mu\nu\alpha\beta}$
\end{itemize}

\begin{align}
    \Tr\qty[\gamma_5\gamma^\mu\gamma^\nu\gamma^\alpha\gamma^\beta]
\end{align}

This is a little bit more complicated, but we can use some tricks, we see that if we have two or more indices 
equal it gives zero, due to the last property,

\begin{align}
    \Tr\qty[\gamma_5\gamma^\mu\gamma^\mu\gamma^\alpha\gamma^\beta]&=g^{\mu\mu}\Tr\qty[\gamma_5\gamma^\alpha\gamma^\beta]=0\nonumber
\end{align}

Hence it can only be non-zero when all indices are different from each other. in this case, as the Gamma matrices 
anticommute with each other, that is, this quantity is totally antisymmetric in all indices, thus, it must 
be proportional to `$\epsilon^{\mu\nu\alpha\beta}$' as this is the only fully antisymmetric quantity in `$4$' 
dimensions,

\begin{align}
    \Tr\qty[\gamma_5\gamma^\mu\gamma^\mu\gamma^\alpha\gamma^\beta]&\propto\epsilon^{\mu\nu\alpha\beta}\nonumber\\
    \Tr\qty[\gamma_5\gamma^0\gamma^1\gamma^2\gamma^3]&\propto\epsilon^{0123}\nonumber\\
    \im\Tr\qty[\gamma^0\gamma^1\gamma^2\gamma^3\gamma^0\gamma^1\gamma^2\gamma^3]&\propto-1\nonumber\\
    -\im\Tr\qty[\gamma^0\gamma^0\gamma^1\gamma^2\gamma^3\gamma^1\gamma^2\gamma^3]&\propto-1\nonumber\\
    \im\Tr\qty[\gamma^1\gamma^1\gamma^2\gamma^3\gamma^2\gamma^3]&\propto-1\nonumber\\
    -\im\Tr\qty[\gamma^2\gamma^2\gamma^3\gamma^3]&\propto-1\nonumber\\
    -4\im&\propto-1\nonumber\\
\end{align}

Hence,

\begin{align}
    \Tr\qty[\gamma_5\gamma^\mu\gamma^\mu\gamma^\alpha\gamma^\beta]&=4\im\epsilon^{\mu\nu\alpha\beta}\nonumber
\end{align}

Now we got for some other equalities,

\begin{itemize}
    \item $\qty(\gamma^\mu)^2=g^{\mu\mu}$
\end{itemize}

\begin{align}
    \acomm{\gamma^\mu}{\gamma^\mu}&=2g^{\mu\mu}\nonumber\\
    2\gamma^\mu=2g^{\mu\mu}\nonumber\\
    \qty(\gamma^\mu)^2&=g^{\mu\mu}\nonumber
\end{align} 

\begin{itemize}
    \item $\gamma_\mu\gamma^\mu=D$
\end{itemize}

\begin{align}
    g_{\mu\nu}\acomm{\gamma^\mu}{\gamma^\nu}&=2g_{\mu\nu}g^{\mu\nu}\nonumber\\
    2\gamma_\mu\gamma^\mu&=2D\nonumber\\
    \gamma_\mu\gamma^\mu&=D\nonumber
\end{align}

\begin{itemize}
    \item $\gamma_\mu\gamma^\alpha\gamma^\mu=\qty(2-D)\gamma^\alpha$
\end{itemize}

\begin{align}
    \gamma_\mu\gamma^\alpha\gamma^\mu&=\gamma_\mu\qty(-\gamma^\mu\gamma^\alpha+2g^{\mu\alpha})\nonumber\\
    &=-\gamma_\mu\gamma^\mu\gamma^\alpha+2\gamma^\alpha\nonumber\\
    &=\qty(2-D)\gamma^\alpha
\end{align}

\begin{itemize}
    \item $\gamma_\mu\gamma^\alpha\gamma^\beta\gamma^\mu=\qty(D-2)\gamma^\alpha\gamma^\beta+2\gamma^\beta\gamma^\alpha$
\end{itemize}

\begin{align}
    \gamma_\mu\gamma^\alpha\gamma^\beta\gamma^\mu&=\gamma_\mu\gamma^\alpha\qty(-\gamma^\mu\gamma^\beta+2g^{\beta\mu})\nonumber\\
    &=-\gamma_\mu\gamma^\alpha\alpha\gamma^\mu\gamma^\beta+\gamma^\beta\gamma^\alpha\nonumber\\
    &=\qty(D-2)\gamma^\alpha\gamma^\beta+2\gamma^\beta\gamma^\alpha\nonumber
\end{align}

\begin{itemize}
    \item $\gamma_\mu\gamma^\alpha\gamma^\beta\gamma^\delta\gamma^\mu=+2\gamma_\delta\gamma^\alpha\gamma^\beta-2\gamma^\beta\gamma^\alpha\gamma^\delta+\qty(2-D)\gamma^\alpha\gamma^\beta\gamma^\delta$
\end{itemize}

\begin{align}
    \gamma_\mu\gamma^\alpha\gamma^\beta\gamma^\delta\gamma^\mu&=
    \gamma_\mu\gamma^\alpha\gamma^\beta\qty(-\gamma^\mu\gamma^\delta+2g^{\mu\delta})\nonumber\\
    &=-\gamma_\mu\gamma^\alpha\gamma^\beta\gamma^\mu\gamma^\delta+2\gamma_\delta\gamma^\alpha\gamma^\beta\nonumber\\
    &=-\qty(D-2)\gamma^\alpha\gamma^\beta\gamma^\delta-2\gamma^\beta\gamma^\alpha\gamma^\delta+2\gamma_\delta\gamma^\alpha\gamma^\beta\nonumber
\end{align}