\problem{}
\probitem{}

Let's our hypothesis, first the mode expansion,
\begin{align*}
    \partial X\qty(z)&=\sum\limits_{m\in\mathbb Z}\frac{\alpha_m}{z^{m+1}}
\end{align*}
and the algebras,
\begin{align*}
    \comm{L_m}{L_n}&=\qty(m-n)L_{n+m}+\frac{c}{12}m\qty(m^2-1)\delta_{m,-n}\\
    \comm{\alpha_m}{\alpha_n}&=m\delta_{m,-n}\\
    \comm{L_m}{\alpha_n}&=-n\alpha_{n+m}
\end{align*}
that have the followings adjoints,
\begin{align*}
    L^\dagger_n&=L_{-n}\\
    \alpha^{\dagger}_n&=\alpha_{-n}
\end{align*}
with this we define the vacuum state $\Psi_0$ as the unique one which satisfy,
\begin{align*}
    L_n\Psi_0=0,\ \ \ n\geq-1
\end{align*}

Let's analyze the action of $L_0$,
\begin{align*}
    0=L_0\Psi_0&=\qty(\frac12\alpha_0\alpha_0+\sum\limits_{n=1}^\infty\alpha_{-n}\alpha_n)\Psi_0\\
    0=\qty(\Psi_0,L_0\Psi_0)&=\frac12\qty(\Psi_0,\alpha_0\alpha_0\Psi_0)+\sum\limits_{n=1}^\infty\qty(\Psi_0,\alpha_{-n}\alpha_n\Psi_0)\\
    0&=\frac12\qty(\alpha_0\Psi_0,\alpha_0\Psi_0)+\sum\limits_{n=1}^\infty\qty(\alpha_{n}\Psi_0,\alpha_n\Psi_0)\\
    0&=\frac12\norm{\alpha_0\Psi_0}^2+\sum\limits_{n=1}^\infty\norm{\alpha_n\Psi_0}^2
\end{align*}

It's clear, in the right-hand side we have the sum o various norms, which are by definition positive, and in the left-hand side we have zero, 
the only way a sum of non-negative numbers can be zero is if each one is zero, that is,
\begin{align*}
    \norm{\alpha_n\Psi_0}^2=0,\ \ \ \forall n\geq 0
\end{align*}
but, as long as the inner product is non degenerate, a zero norm state is the null/zero state, that means,
\begin{align*}
    \alpha_n\Psi_0=0,\ \ \ \forall n\geq 0
\end{align*}
what is the desired result. Nothing more can be said of $\alpha_n\Psi_0$ for $n<0$ than that at least $\alpha_{-1}\Phi_0$ is non zero for a non trivial theory.

\probitem{}

Start by,
\begin{align*}
    \partial X\qty(z)\partial X\qty(w)&=\textnormal{singular}+\textnormal{regular},\ \ \ \abs{z}>\abs{w}\\
    \qty(\Psi_0,\partial X\qty(z)\partial X\qty(w)\Psi_0)&=\qty(\Psi_0,\textnormal{singular}\Psi_0)+\qty(\Psi_0,\textnormal{regular}\Psi_0),\ \ \ \abs{z}>\abs{w}\\
    \qty(\Psi_0,\partial X\qty(z)\partial X\qty(w)\Psi_0)&=\qty(\Psi_0,\textnormal{singular}\Psi_0),\ \ \ \abs{z}>\abs{w}
\end{align*}
due to the regular part being a normal ordered term. Now, substituting the definition of the normal modes,
\begin{align*}
    \qty(\Psi_0,\textnormal{singular}\Psi_0)&=\qty(\Psi_0,\partial X\qty(z)\partial X\qty(w)\Psi_0),\ \ \ \abs{z}>\abs{w}\\
    \qty(\Psi_0,\textnormal{singular}\Psi_0)&=\sum\limits_{n,m\in\mathbb Z}\frac{1}{z^{n+1}w^{m+1}}\qty(\Psi_0,\alpha_n\alpha_m\Psi_0),\ \ \ \abs{z}>\abs{w}\\
    \qty(\Psi_0,\textnormal{singular}\Psi_0)&=\sum\limits_{n,m\in\mathbb Z}\frac{1}{z^{n+1}w^{m+1}}\delta\qty(m<0)\qty(\alpha_{-n}\Psi_0,\alpha_m\Psi_0),\ \ \ \abs{z}>\abs{w}\\
    \qty(\Psi_0,\textnormal{singular}\Psi_0)&=\sum\limits_{n\in\mathbb Z}\sum\limits_{m<0}\frac{1}{z^{n+1}w^{m+1}}\delta\qty(-n<0)\qty(\alpha_{-n}\Psi_0,\alpha_m\Psi_0),\ \ \ \abs{z}>\abs{w}\\
    \qty(\Psi_0,\textnormal{singular}\Psi_0)&=\sum\limits_{n\in\mathbb Z}\sum\limits_{m<0}\frac{1}{z^{n+1}w^{m+1}}\delta\qty(n>0)\qty(\alpha_{-n}\Psi_0,\alpha_m\Psi_0),\ \ \ \abs{z}>\abs{w}\\
    \qty(\Psi_0,\textnormal{singular}\Psi_0)&=\sum\limits_{n>0}\sum\limits_{m<0}\frac{1}{z^{n+1}w^{m+1}}\qty(\alpha_{-n}\Psi_0,\alpha_m\Psi_0),\ \ \ \abs{z}>\abs{w}\\
    \qty(\Psi_0,\textnormal{singular}\Psi_0)&=\sum\limits_{m,n<0}\frac{1}{z^{n+1}w^{m+1}}\qty(\alpha_{n}\Psi_0,\alpha_m\Psi_0),\ \ \ \abs{z}>\abs{w}\\
    \qty(\Psi_0,\textnormal{singular}\Psi_0)&=\sum\limits_{m,n<0}\frac{1}{z^{n+1}w^{m+1}}\qty(\Psi_0,\alpha_{-n}\alpha_m\Psi_0),\ \ \ \abs{z}>\abs{w}\\
    \qty(\Psi_0,\textnormal{singular}\Psi_0)&=\sum\limits_{m,n<0}\frac{1}{z^{n+1}w^{m+1}}\qty(\Psi_0,\qty(\alpha_{-n}\alpha_m-\alpha_m\alpha_{-n}+\alpha_m\alpha_{-n})\Psi_0),\ \ \ \abs{z}>\abs{w}\\
    \qty(\Psi_0,\textnormal{singular}\Psi_0)&=\sum\limits_{m,n<0}\frac{1}{z^{n+1}w^{m+1}}\qty(\Psi_0,\qty(\comm{\alpha_{-n}}{\alpha_m}+\alpha_m\alpha_{-n})\Psi_0),\ \ \ \abs{z}>\abs{w}\\
    \qty(\Psi_0,\textnormal{singular}\Psi_0)&=\sum\limits_{m,n<0}\frac{1}{z^{n+1}w^{m+1}}\qty(\Psi_0,\qty(-n\delta_{m,n}+\delta\qty(-n<0)\alpha_m\alpha_{-n})\Psi_0),\ \ \ \abs{z}>\abs{w}\\
    \qty(\Psi_0,\textnormal{singular}\Psi_0)&=\sum\limits_{m,n<0}\frac{1}{z^{n+1}w^{m+1}}\qty(-n)\delta_{m,n}\qty(\Psi_0,\Psi_0),\ \ \ \abs{z}>\abs{w}\\
    \qty(\Psi_0,\textnormal{singular}\Psi_0)&=\sum\limits_{n<0}\frac{1}{z^{n+1}w^{n+1}}\qty(-n)\qty(\Psi_0,\Psi_0),\ \ \ \abs{z}>\abs{w}\\
    \qty(\Psi_0,\textnormal{singular}\Psi_0)&=-\sum\limits_{n<0}nz^{-n-1}w^{-n-1}\qty(\Psi_0,\Psi_0),\ \ \ \abs{z}>\abs{w}\\
    \qty(\Psi_0,\textnormal{singular}\Psi_0)&=\frac{1}{zw}\sum\limits_{n>0}n\qty(zw)^{n}\qty(\Psi_0,\Psi_0),\ \ \ \abs{z}>\abs{w}
\end{align*}

This power series has a nice representation,
\begin{align*}
    \sum\limits_{n>0}nx^n&=\frac{x}{\qty(x-1)^2},\ \ \ \abs{x}<1
\end{align*}
so,
\begin{align*}
    \qty(\Psi_0,\textnormal{singular}\Psi_0)&=\frac{1}{zw}\qty(\Psi_0,\Psi_0)\frac{zw}{\qty(zw-1)^2},\ \ \ \abs{z}>\abs{w},\ \abs{zw}<1\\
    \qty(\Psi_0,\textnormal{singular}\Psi_0)&=\qty(\Psi_0,\Psi_0)\frac{1}{\qty(zw-1)^2},\ \ \ \abs{z}>\abs{w},\ \abs{zw}<1
\end{align*}
but, $\qty(\Psi_0,\Psi_0)=1$,
\begin{align*}
    \qty(\Psi_0,\textnormal{singular}\Psi_0)&=\frac{1}{\qty(zw-1)^2},\ \ \ \abs{z}>\abs{w},\ \abs{zw}<1
\end{align*}

The OPE is then,
\begin{align*}
    \partial X\qty(z)\partial X\qty(w)&=\frac{1}{\qty(zw-1)^2}+\textnormal{regular},\ \ \ \abs{z}>\abs{w},\ \abs{zw}<1
\end{align*}